TEMP0

theories/interp.v
@@ -5,12 +5,72 @@
  * LICENSE file in the root directory of this source tree.
  *)
 From stdpp Require Import base strings gmap stringmap fin_maps natmap list.
+
+Section MissingHelpers.
+  Context {A B: Type} (f: A → B).
+
+  Lemma list_fmap_equiv_ext_elem_of `{!Equiv B} (g : A → B) l :
+        (∀ x, x ∈ l → f x ≡ g x) → f <$> l ≡ g <$> l.
+  Proof.
+    induction l as [ | hd tl hi]; intro h; simpl in *.
+    { by constructor. }
+    f_equiv.
+    { apply h; by constructor. }
+    apply hi; intros x hin.
+    apply h; by constructor.
+  Qed.
+End MissingHelpers.
+
+
 From iris.base_logic Require Import upred derived.
 From iris.base_logic.lib Require Import iprop own.
 From iris.algebra Require Import ofe cmra gmap_view.
 From iris.proofmode Require Import tactics.
 
 From shack Require Import lang progdef subtype typing eval heap modality.
+
+Section Helpers.
+  Context { Σ: gFunctors }.
+
+  Fixpoint iForall3 {A B C : Type} (P : A → B → C → iProp Σ)
+    (As : list A) (Bs: list B) (Cs : list C) {struct As}  : iProp Σ :=
+    match As, Bs, Cs with
+    | [], [], [] => True%I
+    | A :: As, B :: Bs, C :: Cs => (P A B C ∗ iForall3 P As Bs Cs)%I
+    | _, _, _ => False%I
+    end.
+
+  Lemma iForall3_length {A B C : Type} (P: A → B → C → iProp Σ)
+     As Bs Cs: ⊢ iForall3 P As Bs Cs → ⌜length As = length Bs ∧ length Bs = length Cs⌝.
+  Proof.
+    revert Bs Cs.
+    induction As as [ | a As hi];
+      case => [ | b Bs];
+      case => [ | c Cs]; iIntros "h" => //=.
+    iDestruct "h" as "[_ h]".
+    iDestruct (hi with "h") as "%h".
+    by destruct h as [-> ->].
+  Qed.
+
+  Lemma iForall3_forall_1 {A B C : Type} (P: A → B → C → iProp Σ)
+     As Bs Cs: ⊢ iForall3 P As Bs Cs →
+     ∀ k a b c, ⌜As !! k = Some a⌝ → ⌜Bs !! k = Some b⌝ → ⌜Cs !! k = Some c⌝ →
+     P a b c.
+  Proof.
+    revert Bs Cs.
+    induction As as [ | a As hi];
+      case => [ | b Bs];
+      case => [ | c Cs]; iIntros "h" (k u v w hu hv hw)=> //=.
+    destruct k as [ | k].
+    - case: hu => ->.
+      case: hv => ->.
+      case: hw => ->.
+      by iDestruct "h" as "[? ?]".
+    - iDestruct "h" as "[_ h]".
+      iDestruct ((hi Bs Cs) with "h") as "h".
+      by iApply "h".
+  Qed.
+End Helpers.
 
 (* the interpretation of types is simply given by
      the carrier set of the sem_typeO ofe *)
@@ -83,9 +143,7 @@ Section proofs.
   (* now, let's interpret some types ! *)
 
   (* Most interpretation functions are parametrized by Σi: tvar -> interp
-   * and Σc: list constraint.
    * Σi is here to interpret generic types.
-   * Σc is there to put constraints on generic types.
    *
    * We could only consider closed types and eagerly apply all top level
    * substitution, but this way makes things a bit more compositional.
@@ -108,83 +166,82 @@ Section proofs.
   Definition interp_nothing : interp Σ :=
     Interp (λ (_: value), False%I).
 
-  Notation ty_interpO := (lang_ty -d> interpO Σ).
+  Notation ty_interpO := (lang_ty -d> listO (interpO Σ) -n> interpO Σ).
 
-  Variable Σc : list constraint.
-  Variable Σi : list (interp Σ).
-
-  Definition interp_fields
-    (C: tag)
-    σC
-    (dom_fields: stringset)
-    (ifields: gmapO string (laterO (sem_typeO Σ)))
-    (rec: ty_interpO) : iProp Σ :=
-    (⌜dom ifields = dom_fields⌝ ∗
-    (∀ f vis ty orig, ⌜has_field f C vis ty orig⌝ -∗ ifields !! f ≡ Some (Next (interp_car (rec (subst_ty σC ty)))))
-    )%I.
-
-  Definition interp_class C σC (rec : ty_interpO) : interp Σ :=
-    Interp (
-      λ (w : value),
-      (∃ ℓ t cdef σ σt (fields: stringmap ((visibility * lang_ty) * tag)) (ifields: gmapO string (laterO (sem_typeO Σ))),
-      ⌜w = LocV ℓ ∧
-       inherits_using t C σ ∧
-       wf_ty (ClassT t σt) ∧
-       ok_ty Σc (ClassT t σt) ∧
-       Δ !! C = Some cdef ∧
-
-       Σc ⊢ (subst_ty σt <$> σ) <: cdef.(generics) :> σC ∧
-
-       has_fields t fields⌝ ∗
-      interp_fields t σt (dom fields) ifields rec ∗
-      (ℓ ↦ (t, ifields)))%I
-    ).
-
-  Definition interp_class_strict C σC (rec : ty_interpO) : interp Σ :=
-    Interp (
-      λ (w : value),
-      (∃ ℓ t σ σt (fields: stringmap ((visibility * lang_ty) * tag)) (ifields: gmapO string (laterO (sem_typeO Σ))),
-      ⌜w = LocV ℓ ∧ inherits_using t C σ ∧
-       wf_ty (ClassT t σt) ∧ ok_ty Σc (ClassT t σt) ∧
-       (subst_ty σt <$> σ) = σC ∧
-       has_fields t fields⌝ ∗
-      interp_fields t σt (dom fields) ifields rec ∗
-      (ℓ ↦ (t, ifields)))%I
-    ).
-
-  Lemma interp_class_from_strict C σC (rec: ty_interpO) v:
-    map_Forall (λ _cname, wf_cdef_parent Δ) Δ →
-    interp_class_strict C σC rec v -∗ interp_class C σC rec v.
+  Lemma ty_interpO_ne : ∀ (rec: ty_interpO) ty, NonExpansive (rec ty).
   Proof.
-    iIntros (hp) "H".
-    iDestruct "H" as (??????) "[%hpure [Hfields Hl]]".
-    destruct hpure as (-> & hin & hwf & hok & heqp & hfs).
-    assert (hin' := hin).
-    apply inherits_using_wf in hin' => //.
-    destruct hin' as (def & ? & ? & hwfC); inv hwfC; simplify_eq.
-    iExists _, _, def0, _, _, _, _.
-    iSplit; last by iSplit.
-    iPureIntro.
-    repeat split => //.
-    apply subtype_targs_refl.
-    by rewrite map_length.
+    move => rec ty.
+    apply _.
   Qed.
 
-  Definition interp_ex (cname: tag) (rec: ty_interpO): interp Σ :=
-    Interp (λ (w: value), (∃ σc, ⌜wf_ty (ClassT cname σc)⌝ ∗ interp_class cname σc rec w)%I).
+  Definition interp_variance (v: variance) (i0 i1: interp Σ) : iProp Σ :=
+    match v with
+    | Invariant => ∀ w, i0 w ∗-∗ i1 w
+    | Covariant => ∀ w, i0 w -∗ i1 w
+    | Contravariant => ∀ w, i1 w -∗ i0 w
+    end.
+
+  (* See
+   * https://gitlab.mpi-sws.org/iris/iris/-/blob/master/iris/base_logic/lib/invariants.v#L10
+   * for example about `seal`.
+   *)
+  Definition interp_tag_def
+    (rec : ty_interpO)
+    (Σi : list (interp Σ))
+    (C: tag)
+    : interp Σ :=
+    Interp (
+      λ (w : value), (∃ ℓ t cdef σ (Σt: list (interp Σ))
+       (fields: stringmap ((visibility * lang_ty) * tag))
+       (ifields: gmapO string (laterO (sem_typeO Σ))),
+      ⌜w = LocV ℓ ∧
+       Δ !! C = Some cdef ∧
+       inherits_using t C σ ∧
+       has_fields t fields ∧
+       dom fields = dom ifields⌝ ∗
+
+       □ ▷ (∀ k v i0 i1,
+         ⌜cdef.(generics) !! k = Some v⌝ →
+         ((λ ty, rec ty Σt) <$> σ) !! k ≡ Some i0 →
+         Σi !! k ≡ Some i1 →
+         interp_variance v i0 i1) ∗
+
+      (∀ f vis ty orig, ⌜has_field f t vis ty orig⌝ -∗
+        ifields !! f ≡ Some (Next (interp_car (rec ty Σt)))) ∗
+
+      (ℓ ↦ (t, ifields)))%I
+    ).
+
+   Local Definition interp_tag_aux
+     (rec : ty_interpO) (Σi : list (interp Σ)) (C: tag)
+     : seal (@interp_tag_def rec Σi C).
+   Proof. by eexists. Qed.
+
+   Definition interp_tag (rec: ty_interpO) (Σi: list (interp Σ)) (C: tag) :=
+     (interp_tag_aux rec Σi C).(unseal).
+
+   Definition interp_tag_unseal 
+     (rec : ty_interpO) (Σi : list (interp Σ)) (C: tag)
+     : interp_tag rec Σi C = interp_tag_def rec Σi C :=
+     (interp_tag_aux rec Σi C).(seal_eq).
+
+  Definition interp_ex (rec: ty_interpO) C : interp Σ :=
+    Interp (λ (w: value),
+      (∃ Σi cdef, ⌜Δ !! C = Some cdef ∧ length Σi = length cdef.(generics)⌝ ∗
+      interp_tag rec Σi C w)%I).
 
   Definition interp_nonnull (rec : ty_interpO) : interp Σ :=
     Interp (
       λ (v : value),
       ((interp_int v) ∨
       (interp_bool v) ∨
-      (∃ t, interp_ex t rec v))%I
+      (∃ t, interp_ex rec t v))%I
     ).
 
   Definition interp_mixed (rec: ty_interpO) : interp Σ :=
     Interp (λ (v: value), (interp_nonnull rec v ∨ interp_null v)%I).
 
-  Definition interp_generic (tv: nat) : interp Σ :=
+  Definition interp_generic (Σi : list (interp Σ)) (tv: nat) : interp Σ :=
     default interp_nothing (Σi !! tv).
 
   (* we use a blend of Coq/Iris recursion, the
@@ -195,50 +252,94 @@ Section proofs.
   Section interp_type_pre_rec.
     Variable (rec: ty_interpO).
 
-    Fixpoint go (typ: lang_ty) : interp Σ :=
+    Fixpoint go (Σi: listO (interpO Σ)) (typ: lang_ty) : interp Σ :=
       match typ with
       | IntT => interp_int
       | BoolT => interp_bool
       | NothingT => interp_nothing
       | MixedT => interp_mixed rec
-      | ClassT A σA => interp_class A σA rec
+      | ClassT A σA =>
+          let Σi := (go Σi) <$> σA in
+          interp_tag rec Σi A
       | NullT => interp_null
       | NonNullT => interp_nonnull rec
-      | UnionT A B => interp_union (go A) (go B)
-      | InterT A B => interp_inter (go A) (go B)
-      | GenT n => interp_generic n
-      | ExT cname => interp_ex cname rec
+      | UnionT A B => interp_union (go Σi A) (go Σi B)
+      | InterT A B => interp_inter (go Σi A) (go Σi B)
+      | GenT n => interp_generic Σi n
+      | ExT cname => interp_ex rec cname
       end.
   End interp_type_pre_rec.
 
-  (* TODO: find a better name for go *)
-  Definition interp_type_pre (rec : ty_interpO) : ty_interpO :=
-    λ (typ : lang_ty), go rec typ.
-
-  Global Instance interp_type_pre_persistent (rec: ty_interpO) :
-    ∀ t v, Persistent (interp_type_pre rec t v).
-  Proof. by move => ??; apply _. Qed.
-
-  Global Instance interp_class_contractive cname σc:
-    Contractive (interp_class cname σc).
+ Local Instance interp_tag_ne C (rec: ty_interpO) :
+    NonExpansive (λ Σi, interp_tag rec Σi C).
   Proof.
-    rewrite /interp_class => n i1 i2 hdist v.
-    rewrite /interp_fun !interp_car_simpl.
-    do 7 (f_equiv; intros ?).
-    f_equiv.
-    rewrite /interp_fields.
-    do 13 f_equiv.
-    f_contractive.
-    apply interp_car_ne2.
-    by f_equiv.
+    move => n x y h.
+    rewrite !interp_tag_unseal /interp_tag_def => v.
+    rewrite /interp_fun !interp_car_simpl /interp_variance.
+    by repeat f_equiv.
   Qed.
 
-  Global Instance interp_ex_contractive cname: Contractive (interp_ex cname).
+  Local Instance go_ne (rec: ty_interpO) (ty: lang_ty) :
+    NonExpansive (λ Σi, go rec Σi ty).
+  Proof.
+    induction ty as [ | | | | A σ hi | | | A B hA hB | A B hA hB | i | cname ] => //= n x y h.
+    - apply interp_tag_ne.
+      rewrite Forall_forall in hi.
+      apply list_dist_lookup => k.
+      rewrite !list_lookup_fmap.
+      destruct (σ !! k) as [ ty | ] eqn:hty => //=.
+      f_equiv.
+      apply hi => //.
+      by apply elem_of_list_lookup_2 in hty.
+    - rewrite /interp_union => v.
+      rewrite /interp_fun !interp_car_simpl.
+      f_equiv.
+      + revert v; by apply hA.
+      + revert v; by apply hB.
+    - rewrite /interp_inter => v.
+      rewrite /interp_fun !interp_car_simpl.
+      f_equiv.
+      + revert v; by apply hA.
+      + revert v; by apply hB.
+    - rewrite /interp_generic => v.
+      assert (hl: length x = length y) by now apply Forall2_length in h.
+      elim : x y i h hl => [ | hd tl hi]; case => [ | hd' tl'] i h /= hl => //.
+      apply Forall2_cons in h as [hhd htl].
+      case: i hi => [ | i ] hi //=.
+      apply:  hi; first done.
+      by lia.
+  Qed.
+
+  Definition interp_type_pre (rec : ty_interpO) : ty_interpO :=
+    λ (typ : lang_ty), λne (Σi: listO (interpO Σ)), go rec Σi typ.
+
+  Global Instance interp_type_pre_persistent (rec: ty_interpO) :
+    ∀ t σi v, Persistent (interp_type_pre rec t σi v).
+  Proof. by move => ???; apply _. Qed.
+
+  Global Instance interp_tag_contractive Σi C:
+    Contractive (λ rec, interp_tag rec Σi C). 
+  Proof.
+    move => n x y h.
+    rewrite !interp_tag_unseal /interp_tag_def => v.
+    rewrite /interp_fun !interp_car_simpl /interp_variance.
+    do 16 f_equiv.
+    - f_equiv; f_contractive.
+      do 12 f_equiv.
+      apply Forall2_fmap, Forall_Forall2_diag, Forall_forall => ? hin.
+      f_equiv.
+      by  f_equiv.
+    - do 12 f_equiv.
+      f_contractive.
+      by repeat f_equiv.
+  Qed.
+
+  Global Instance interp_ex_contractive C: Contractive (λ rec, interp_ex rec C).
   Proof.
     rewrite /interp_ex => n i1 i2 hdist v.
     rewrite /interp_fun !interp_car_simpl.
-    do 3 f_equiv.
-    by apply interp_class_contractive.
+    do 5 f_equiv.
+    by apply interp_tag_contractive.
   Qed.
 
   Global Instance interp_nonnull_contractive: Contractive interp_nonnull.
@@ -249,14 +350,10 @@ Section proofs.
     by apply interp_ex_contractive.
   Qed.
 
-  (* we cannot use solve_contractive out of the box because of
-   * the 'fix' combinator above
-   *)
   Local Instance interp_type_pre_contractive : Contractive interp_type_pre.
   Proof.
-    rewrite /interp_type_pre => n rec1 rec2 hdist ty /=.
-    induction ty
-      as [ | | | | cname σ hi | | | A B hA hB | A B hA hB | i | cname ] => /=.
+    rewrite /interp_type_pre => n rec1 rec2 hdist ty Σi /=.
+    induction ty as [ | | | | C σ hi | | | A B hA hB | A B hA hB | i | C ] => /=.
     - done.
     - done.
     - done.
@@ -264,11 +361,30 @@ Section proofs.
       rewrite /interp_fun !interp_car_simpl.
       f_equiv.
       revert v; by apply interp_nonnull_contractive.
-    - by apply interp_class_contractive.
+    - rewrite !interp_tag_unseal /interp_tag_def => v.
+      rewrite /interp_fun !interp_car_simpl /interp_variance.
+      rewrite Forall_forall in hi.
+			do 16 f_equiv.
+      + f_equiv; f_contractive.
+        do 10 f_equiv.
+        * do 2 f_equiv.
+          apply Forall2_fmap, Forall_Forall2_diag, Forall_forall => ? hin.
+          f_equiv.
+          by  f_equiv.
+        * do 2 f_equiv.
+          rewrite !list_lookup_fmap.
+          destruct (σ !! a6) as [ ty | ] eqn:hty => //=.
+          f_equiv.
+          apply dist_S.
+          apply hi.
+          by apply elem_of_list_lookup_2 in hty. 
+      + do 12 f_equiv.
+        f_contractive.
+        by apply hdist.
     - done.
     - by apply interp_nonnull_contractive.
-    - solve_proper_core ltac:(fun _ => first [done | f_contractive | f_equiv]).
-    - solve_proper_core ltac:(fun _ => first [done | f_contractive | f_equiv]).
+    - by solve_proper_core ltac:(fun _ => first [done | f_contractive | f_equiv]).
+    - by solve_proper_core ltac:(fun _ => first [done | f_contractive | f_equiv]).
     - done.
     - by apply interp_ex_contractive.
   Qed.
@@ -278,454 +394,866 @@ Section proofs.
      can be (mutually) recursive) *)
   Definition interp_type := fixpoint interp_type_pre.
 
-  (* Helper lemmas to control unfolding of some definitions *)
-  Lemma interp_type_unfold (ty : lang_ty) (v : value) :
-    interp_type ty v ⊣⊢ interp_type_pre interp_type ty v.
-  Proof.
-    rewrite {1}/interp_type.
-    apply (fixpoint_unfold interp_type_pre ty v).
-  Qed.
+  Section Unfold.
+    Variable Σi : list (interpO Σ).
 
-  Lemma interp_ex_unfold t v:
-    interp_type (ExT t) v ⊣⊢ interp_ex t interp_type v.
-  Proof. by rewrite interp_type_unfold /= /interp_ex /=. Qed.
+    (* Helper lemmas to control unfolding of some definitions *)
+    Lemma interp_type_unfold (ty : lang_ty) (v : value) :
+      interp_type ty Σi v ⊣⊢ interp_type_pre interp_type ty Σi v.
+    Proof.
+      rewrite {1}/interp_type.
+      apply (fixpoint_unfold interp_type_pre ty Σi v).
+    Qed.
 
-  Lemma interp_nonnull_unfold v:
-    interp_type NonNullT v ⊣⊢
-      (interp_int v) ∨ (interp_bool v) ∨ (∃ t, interp_ex t interp_type v)%I.
-  Proof. by rewrite interp_type_unfold /= /interp_nonnull /=. Qed.
+    Lemma interp_ex_unfold t v:
+      interp_type (ExT t) Σi v ⊣⊢ interp_ex interp_type t v.
+    Proof. by rewrite interp_type_unfold /= /interp_ex /=. Qed.
 
-  Lemma interp_mixed_unfold v:
-    interp_type MixedT v ⊣⊢ interp_nonnull interp_type v ∨ interp_null v.
-  Proof. by rewrite interp_type_unfold /interp_mixed /=. Qed.
+    Lemma interp_nonnull_unfold v:
+      interp_type NonNullT Σi v ⊣⊢
+      (interp_int v) ∨ (interp_bool v) ∨ (∃ t, interp_ex interp_type t v)%I.
+    Proof. by rewrite interp_type_unfold /= /interp_nonnull /=. Qed.
 
-  Lemma interp_class_unfold A σA v:
-    interp_type (ClassT A σA) v ⊣⊢
-    interp_class A σA interp_type v.
-  Proof. by rewrite interp_type_unfold. Qed.
+    Lemma interp_mixed_unfold v:
+      interp_type MixedT Σi v ⊣⊢ interp_nonnull interp_type v ∨ interp_null v.
+    Proof. by rewrite interp_type_unfold /interp_mixed /=. Qed.
 
-  Lemma interp_union_unfold A B v:
-    interp_type (UnionT A B) v ⊣⊢
-    interp_union (interp_type A) (interp_type B) v.
-  Proof.
-    rewrite interp_type_unfold /=.
+    Lemma interp_union_unfold A B v:
+      interp_type (UnionT A B) Σi v ⊣⊢
+      interp_union (interp_type A Σi) (interp_type B Σi) v.
+    Proof.
+      rewrite interp_type_unfold /=.
     iSplit; iIntros "[H | H]".
     - iLeft; by rewrite interp_type_unfold.
     - iRight; by rewrite interp_type_unfold.
     - iLeft; by rewrite interp_type_unfold.
     - iRight; by rewrite interp_type_unfold.
-  Qed.
+    Qed.
 
-  Lemma interp_inter_unfold A B v:
-    interp_type (InterT A B) v ⊣⊢
-    interp_inter (interp_type A) (interp_type B) v.
-  Proof.
-    rewrite interp_type_unfold /=.
+    Lemma interp_inter_unfold A B v:
+      interp_type (InterT A B) Σi v ⊣⊢
+      interp_inter (interp_type A Σi) (interp_type B Σi) v.
+    Proof.
+      rewrite interp_type_unfold /=.
     iSplit; iIntros "[HL HR]".
     - rewrite !interp_type_unfold; by iSplit.
     - rewrite !interp_type_unfold; by iSplit.
+    Qed.
+  End Unfold.
+
+  Lemma interp_class_unfold Σi A σA v:
+    interp_type (ClassT A σA) Σi v ⊣⊢
+    interp_tag interp_type ((λ ty, interp_type ty Σi) <$> σA) A v.
+  Proof.
+    rewrite interp_type_unfold /=.
+    rewrite !interp_tag_unseal /interp_tag_def.
+    rewrite /interp_fun !interp_car_simpl.
+    do 31 f_equiv.
+    apply list_fmap_equiv_ext => ty w.
+    by rewrite interp_type_unfold.
   Qed.
 
   (* #hyp *)
   Global Instance interp_type_persistent :
-    ∀ t v, Persistent (interp_type t v).
+    ∀ Σi t v, Persistent (interp_type t Σi v).
   Proof.
-    move => t v.
+    move => Σi t v.
     rewrite interp_type_unfold.
     by apply _.
+  Qed.
+
+  Definition interp_list (Σi: list (interp Σ)) (σ: list lang_ty) :=
+    (λ ty, interp_type ty Σi) <$> σ.
+
+  Lemma interp_list_fold Σi σ: go interp_type Σi <$> σ ≡ interp_list Σi σ.
+  Proof.
+    rewrite /interp_list.
+    apply list_fmap_equiv_ext_elem_of => tc htc /= w.
+    by rewrite interp_type_unfold.
+  Qed.
+
+  Lemma interp_list_gen_targs Σi n:
+    length Σi = n →
+    interp_list Σi (gen_targs n) ≡ Σi.
+  Proof.
+    rewrite /interp_list => hlen.
+    apply list_equiv_lookup => k.
+    rewrite list_lookup_fmap.
+    destruct (decide (k < n)) as [hlt | hge].
+    - rewrite (lookup_gen_targs_lt n k) //=.
+      rewrite -hlen in hlt.
+      assert (h: is_Some (Σi !! k)) by by apply lookup_lt_is_Some_2.
+      destruct h as [σi hi].
+      rewrite hi.
+      constructor.
+      move => v.
+      by rewrite interp_type_unfold /= /interp_generic hi.
+    - assert (h: Σi !! k = None).
+      { apply lookup_ge_None_2.
+        by lia.
+      }
+      rewrite h.
+      rewrite /gen_targs list_lookup_fmap lookup_seq_ge //.
+      by lia.
+  Qed.
+
+  Lemma interp_type_subst Σi ty σ v:
+    bounded (length σ) ty →
+    interp_type (subst_ty σ ty) Σi v ≡
+    interp_type ty (interp_list Σi σ) v.
+  Proof.
+    move => hbounded.
+    rewrite !interp_type_unfold; revert v.
+    induction ty as [ | | | | C σC hi | | | A B hA hB | A B hA hB | i | C ] => //= v.
+    - rewrite !interp_tag_unseal /interp_tag_def /= /interp_variance.
+      do 31 f_equiv.
+      rewrite -list_fmap_compose.
+      apply list_fmap_equiv_ext_elem_of => ty hin w.
+      rewrite Forall_forall in hi.
+      apply hi with (v := w) in hin; first by rewrite hin.
+      inv hbounded.
+      rewrite Forall_forall in H0.
+      by apply H0.
+    - inv hbounded; by rewrite hA // hB.
+    - inv hbounded; by rewrite hA // hB.
+    - rewrite /interp_generic list_lookup_fmap.
+      destruct (σ !! i) as [ty | ] eqn:hty => /=.
+      + by rewrite interp_type_unfold.
+      + inv hbounded. 
+        apply lookup_ge_None_1 in hty.
+        by lia.
+  Qed.
+
+  Lemma interp_tag_equivI (Σ0 Σ1: list (interp Σ)):
+    Σ0 ≡ Σ1 →
+    ∀ A v, interp_tag interp_type Σ0 A v ≡ interp_tag interp_type Σ1 A v.
+  Proof.
+    move => h A v.
+    rewrite !interp_tag_unseal /interp_tag_def /interp_variance /=.
+    by repeat f_equiv.
+  Qed.
+
+  Lemma interp_type_equivI (Σ0 Σ1: list (interp Σ)):
+    Σ0 ≡ Σ1 →
+    ∀ ty v, interp_type ty Σ0 v ≡ interp_type ty Σ1 v.
+  Proof.
+    move => hΣ ty v.
+    rewrite !interp_type_unfold; revert v.
+    induction ty as [ | | | | C σC hi | | | A B hA hB | A B hA hB | i | C ] => //= v.
+    - apply interp_tag_equivI.
+      apply list_fmap_equiv_ext_elem_of => ty hin w.
+      rewrite Forall_forall in hi.
+      move: (hi ty hin w).
+      by rewrite /interp_type_pre /= => ->.
+    - by rewrite hA hB.
+    - by rewrite hA hB.
+    - rewrite /interp_generic.
+      assert (hh: (∀ i0 : nat, Σ0 !! i0 ≡ Σ1 !! i0)).
+      { move => j. by rewrite hΣ. }
+      by rewrite (hh i).
+  Qed.
+
+  Lemma neg_interp_variance vs Σ0 Σ1:
+    iForall3 interp_variance vs Σ0 Σ1 -∗
+    iForall3 interp_variance (neg_variance <$> vs) Σ1 Σ0.
+  Proof.
+    revert Σ0 Σ1.
+    induction vs as [ | v vs hi]; intros [ | ty0 Σ0] [ | ty1 Σ1] => //=.
+    iIntros "[hv hi]".
+    iSplitL "hv".
+    - rewrite /interp_variance.
+      destruct v => //=.
+      iIntros (w).
+      iSplit; iSpecialize ("hv" $! w); iIntros "?"; by iApply "hv".
+    - by iApply hi.
+  Qed.
+
+  Lemma interp_with_mono ty vs:
+    map_Forall (λ _ : string, wf_cdef_mono) Δ →
+    map_Forall (λ _ : string, wf_cdef_parent Δ) Δ →
+    ∀ Σ0 Σ1,
+    mono vs ty →
+    wf_ty ty →
+    □ iForall3 interp_variance vs Σ0 Σ1 -∗
+    ∀ v,
+    interp_type ty Σ0 v -∗ interp_type ty Σ1 v.
+  Proof.
+    move => ??.
+    iIntros (Σ0 Σ1 hmono hwf) "#h".
+    iInduction ty as [ | | | | C σC hi | | | A B hA hB | A B hA hB | i | C ] 
+        "IHty" forall (Σ0 Σ1 vs hmono) "h"; iIntros (v); rewrite !interp_type_unfold //=.
+    - by iIntros.
+    - rewrite !interp_tag_unseal /interp_tag_def /interp_fun !interp_car_simpl.
+      iIntros "htag".
+      iDestruct "htag" as (l t cdef σ Σt fields ifields h) "[#hinst [hdyn hloc]]".
+      destruct h as (-> & hcdef & hinherits & hfields & hdom).
+      iExists l, t, cdef, σ, Σt, fields, ifields.
+      iSplitR; first by iPureIntro.
+      iSplitR; last by iSplit.
+      iModIntro; iNext.
+      iDestruct (iForall3_length with "h") as "%hlen".
+      destruct hlen as [hl0 hl1].
+      iIntros (k v i0 i1 hk) "h0 h1".
+      rewrite !list_lookup_fmap.
+      destruct (σ !! k) as [t0 | ] eqn:ht0; last first.
+      { by rewrite !option_equivI. }
+      destruct (σC !! k) as [t1 | ] eqn:ht1; last first.
+      { by rewrite !option_equivI. }
+      rewrite /= !option_equivI.
+      iAssert (iForall3 interp_variance (neg_variance <$> vs) Σ1 Σ0) as "hneg".
+      { by iApply neg_interp_variance. }
+      rewrite /interp_variance.
+      assert (hwf1: wf_ty t1).
+      { inv hwf; simplify_eq.
+        by apply H3 with k.
+      }
+      iAssert (Some (interp_type t0 Σt) ≡ Some (interp_type t0 Σt))%I as "heq0"; first done.
+      iAssert (Some (go interp_type Σ0 t1) ≡ Some (go interp_type Σ0 t1))%I as "heq1"; first done.
+      iSpecialize ("hinst" $! k v (interp_type t0 Σt)  (go interp_type Σ0 t1) hk).
+      rewrite !list_lookup_fmap /= ht0 ht1.
+      iSpecialize ("hinst" with "heq0 heq1").
+      destruct v.
+      + assert (hmono0: mono vs t1).
+        { inv hmono; simplify_eq.
+          by apply H3 with k Invariant.
+        }
+        assert (hmono1: mono (neg_variance <$> vs) t1).
+        { inv hmono; simplify_eq.
+          by apply H4 with k Invariant.
+        }
+        iAssert (□ ∀ w, interp_type t1 Σ0 w -∗ interp_type t1 Σ1 w)%I as "#hc0".
+        { iDestruct (big_sepL_lookup with "IHty") as "#hk"; first by exact ht1.
+          by iApply ("hk" $! hwf1 Σ0 Σ1 _ hmono0 with "h").
+        }
+        iAssert (□ ∀ w, interp_type t1 Σ1 w -∗ interp_type t1 Σ0 w)%I as "#hc1".
+        { iDestruct (big_sepL_lookup with "IHty") as "#hk"; first by exact ht1.
+          by iApply ("hk" $! hwf1 Σ1 Σ0 _ hmono1 with "hneg").
+        }
+        iIntros (w).
+        iRewrite -"h0".
+        iRewrite -"h1".
+        iSplit; iIntros "#?".
+        * iAssert (interp_type t1 Σ1 w) as "hr"; last by rewrite !interp_type_unfold.
+          iApply "hc0".
+          iAssert (go interp_type Σ0 t1 w) as "hh"; last by rewrite !interp_type_unfold.
+          by iApply "hinst".
+        * iApply "hinst".
+          iAssert (interp_type t1 Σ0 w) as "hr"; last by rewrite !interp_type_unfold.
+          iApply "hc1".
+          by rewrite !interp_type_unfold.
+      + assert (hmono0: mono vs t1).
+        { inv hmono; simplify_eq.
+          by apply H3 with k Covariant.
+        }
+        iAssert (□ ∀ w, interp_type t1 Σ0 w -∗ interp_type t1 Σ1 w)%I as "#hc0".
+        { iDestruct (big_sepL_lookup with "IHty") as "#hk"; first by exact ht1.
+          by iApply ("hk" $! hwf1 Σ0 Σ1 _ hmono0 with "h").
+        }
+        iIntros (w).
+        iRewrite -"h0".
+        iRewrite -"h1".
+        iIntros "#?".
+        iAssert (interp_type t1 Σ1 w) as "hr"; last by rewrite !interp_type_unfold.
+        iApply "hc0".
+        iAssert (go interp_type Σ0 t1 w) as "hh"; last by rewrite !interp_type_unfold.
+        by iApply "hinst".
+      + assert (hmono1: mono (neg_variance <$> vs) t1).
+        { inv hmono; simplify_eq.
+          by apply H4 with k Contravariant.
+        }
+        iAssert (□ ∀ w, interp_type t1 Σ1 w -∗ interp_type t1 Σ0 w)%I as "#hc1".
+        { iDestruct (big_sepL_lookup with "IHty") as "#hk"; first by exact ht1.
+          by iApply ("hk" $! hwf1 Σ1 Σ0 _ hmono1 with "hneg").
+        }
+        iIntros (w).
+        iRewrite -"h0".
+        iRewrite -"h1".
+        iIntros "#?".
+        iApply "hinst".
+        iAssert (interp_type t1 Σ0 w) as "hr"; last by rewrite !interp_type_unfold.
+        iApply "hc1".
+        by rewrite !interp_type_unfold.
+    - iIntros "hh".
+      iDestruct "hh" as "[hint | hh]"; first by iLeft.
+      iDestruct "hh" as "[hbool | hh]"; first by (iRight; iLeft).
+      by iRight; iRight.
+    - inv hmono.
+      inv hwf.
+      iIntros "hh".
+      iDestruct "hh" as "[hh | hh]".
+      + iLeft.
+        rewrite -!interp_type_unfold /=.
+        by iApply "IHty".
+      + iRight.
+        rewrite -!interp_type_unfold /=.
+        by iApply "IHty1".
+    - inv hmono.
+      inv hwf.
+      iIntros "hh".
+      iDestruct "hh" as "[h0 h1]".
+      rewrite -!interp_type_unfold /=.
+      iSplit; first by iApply "IHty".
+      by iApply "IHty1".
+    - iDestruct (iForall3_length with "h") as "%hl".
+      destruct hl as [hl0 hl1].
+      destruct (vs !! i) as [vi | ] eqn:hvi; last first.
+      { destruct (Σ0 !! i) as [ ? | ] eqn:h0.
+        { apply lookup_ge_None_1 in hvi.
+          apply lookup_lt_Some in h0.
+          by lia.
+        }
+        destruct (Σ1 !! i) as [ ? | ] eqn:h1.
+        { apply lookup_ge_None_1 in hvi.
+          apply lookup_lt_Some in h1.
+          by lia.
+        }
+        by rewrite /interp_generic h0 h1.
+      }
+      destruct (Σ0 !! i) as [ i0 | ] eqn:h0; last first.
+      { apply lookup_ge_None_1 in h0.
+        apply lookup_lt_Some in hvi.
+        by lia.
+      }
+      destruct (Σ1 !! i) as [ i1 | ] eqn:h1; last first.
+      { apply lookup_ge_None_1 in h1.
+        apply lookup_lt_Some in hvi.
+        by lia.
+      }
+      simpl.
+      iDestruct (iForall3_forall_1 with "h") as "hf".
+      iSpecialize ("hf" $! i vi i0 i1 hvi h0 h1).
+      iClear "h".
+      rewrite /interp_variance.
+      rewrite /interp_generic /= h0 h1 /=.
+      inv hmono; simplify_eq.
+      * iSpecialize ("hf" $! v).
+        by iDestruct "hf" as "[? ?]".
+      * by iSpecialize ("hf" $! v).
+    - iIntros "hh".
+      iDestruct "hh" as (Σt cdef h) "hh".
+      destruct h as [hcdef hlen].
+      iExists Σt, cdef; by iSplit.
+  Qed.
+
+  Lemma tag_extends_using_is_inclusion:
+    map_Forall (λ _cname, wf_cdef_parent Δ) Δ →
+    map_Forall (λ _ : string, wf_cdef_mono) Δ →
+    ∀ A B σB, extends_using A B σB →
+    ∀ Σi v adef,
+    Δ !! A = Some adef →
+    length Σi = length adef.(generics) →
+    interp_tag interp_type Σi A v -∗
+    interp_tag interp_type (interp_list Σi σB) B v.
+  Proof.
+    move => hwp hmono A B σB hext Σi v adef hadef hlen.
+    rewrite !interp_tag_unseal /interp_tag_def /interp_fun !interp_car_simpl.
+    iIntros "h".
+    iDestruct "h" as (ℓ t adef' σ Σt fields ifields) "[%h [#hinst [hdyn hl]]]".
+    destruct h as (-> & hadef' & hin & hfields & hdom); simplify_eq.
+    destruct (extends_using_wf _ _ _ hwp hext) as (adef' & hadef' & hF & hwfB).
+    destruct (inherits_using_wf _ _ _ hwp hin) as (tdef & htdef & htF & hwfA).
+    simplify_eq.
+    assert (hb: is_Some (Δ !! B)) by by inv hwfB.
+    destruct hb as [bdef hbdef].
+    iExists ℓ, t, bdef, (subst_ty σ <$> σB), Σt, fields, ifields.
+    iSplit.
+    { iPureIntro; repeat split => //.
+      by eapply inherits_using_trans; last by econstructor.
+    }
+    iSplitR; last by iSplit.
+    iModIntro; iNext.
+    iIntros (k v i0 i1 hv) "h0 h1".
+    destruct (σB !! k) as [tb | ] eqn:htb; last first.
+    { by rewrite !list_lookup_fmap htb /= !option_equivI. }
+    assert (h := hadef).
+    apply hmono in h.
+    rewrite /wf_cdef_mono in h.
+    destruct hext as [A B adef' σB hadef' hsuper]; simplify_eq.
+    rewrite hsuper in h.
+    inv h; simplify_eq.
+    specialize (H4 k v tb hv htb).
+    specialize (H3 k v tb hv htb).
+    rewrite !list_lookup_fmap htb /= !option_equivI.
+    assert (hσ : length σ = length adef'.(generics)).
+    { inv hwfA; by simplify_eq. }
+    assert (wftb: wf_ty tb).
+    { inv hwfB; simplify_eq.
+      by eauto.
+    }
+    assert (hboundedtb:  bounded (length σ) tb).
+    { rewrite Forall_forall in hF.
+      rewrite hσ.
+      apply hF.
+      by apply elem_of_list_lookup_2 in htb.
+    }
+    iAssert (□ iForall3 interp_variance adef'.(generics) (interp_list Σt σ) Σi)%I as "hf0".
+    { iModIntro.
+      move: hlen hσ.
+      generalize (generics adef') => l.
+      clear.
+      move => hlen hσ.
+      iInduction l as [ | hd tl] "HI" forall (σ Σi hlen hσ).
+      { by destruct σ; destruct Σi. }
+      destruct σ as [ | ty σ] => //=.
+      destruct Σi as [ | ii Σi] => //=.
+      case: hlen => hlen.
+      case: hσ => hσ.
+      iSplitL; first by iApply ("hinst" $! 0).
+      iApply "HI" => //.
+      iModIntro; iIntros (k v i0 i1 hk) "#h0 #h1".
+      by iApply ("hinst" $! (S k)).
+    }
+    iAssert (□ iForall3 interp_variance (neg_variance <$> adef'.(generics)) Σi (interp_list Σt σ))%I as "hf1".
+    { by iModIntro; iApply neg_interp_variance. }
+    iClear "hinst".
+    destruct v.
+    - assert (hmono0 : mono (generics adef') tb) by by apply H3.
+      assert (hmono1 : mono (neg_variance <$> generics adef') tb) by by apply H4.
+      rewrite /interp_variance /=; iIntros (w).
+      iRewrite -"h0".
+      iRewrite -"h1".
+      iSplit; iIntros "#?".
+      + iApply (interp_with_mono with "hf0") => //.
+        by rewrite interp_type_subst.
+      + rewrite interp_type_subst //.
+        by iApply (interp_with_mono with "hf1").
+    - assert (hmono0 : mono (generics adef') tb) by by apply H3.
+      rewrite /interp_variance /=; iIntros (w).
+      iRewrite -"h0".
+      iRewrite -"h1".
+      iIntros "#?".
+      iApply (interp_with_mono with "hf0") => //.
+      by rewrite interp_type_subst.
+    - assert (hmono1 : mono (neg_variance <$> generics adef') tb) by by apply H4.
+      rewrite /interp_variance /=; iIntros (w).
+      iRewrite -"h0".
+      iRewrite -"h1".
+      iIntros "#?".
+      rewrite interp_type_subst //.
+      by iApply (interp_with_mono with "hf1").
   Qed.
 
   (* if class A<..> extends B<σB>, then for any valid substitution σA,
    * [| A<σA> |] ⊆ [| B<σA o σB> |]
    *)
   Lemma extends_using_is_inclusion:
-    map_Forall (λ _cname, wf_cdef_fields) Δ →
-    map_Forall (λ _cname, wf_cdef_fields_bounded) Δ →
     map_Forall (λ _cname, wf_cdef_parent Δ) Δ →
-    map_Forall (λ _cname, wf_cdef_mono) Δ →
-    ∀ A B σB, extends_using A B σB →
-    ∀ v σA, Forall wf_ty σA →
-    interp_type (ClassT A σA) v -∗
-    interp_type (ClassT B (subst_ty σA <$> σB)) v.
+    map_Forall (λ _ : string, wf_cdef_mono) Δ →
+    ∀ Σi A B σA σB v, extends_using A B σB →
+    wf_ty (ClassT A σA) →
+    interp_type (ClassT A σA) Σi v -∗
+    interp_type (ClassT B (subst_ty σA <$> σB)) Σi v.
   Proof.
-    move => hwf hwfb hwp hmono A B σB hext v σA hwfσA.
-    rewrite !interp_type_unfold /=.
+    move => ?? Σi A B σA σB v hext hwfA.
+    rewrite !interp_class_unfold.
     iIntros "h".
-    iDestruct "h" as (ℓ t adef σ σt fields ifields) "[%h [hsem hl]]".
-    destruct h as (-> & hin & hσwf & hσok & hadef & hσ & hfields).
-    destruct (extends_using_wf _ _ _ hwp hext) as (adef' & hadef' & hF & hwfB).
-    simplify_eq.
-    assert (hwfσt : Forall wf_ty σt) by (by apply wf_ty_class_inv in hσwf).
-    assert (hwfσ : Forall wf_ty σ).
-    { apply inherits_using_wf in hin => //.
-      destruct hin as (? & ? & ? &h).
-      by apply wf_ty_class_inv in h.
+    assert (hΣ : interp_list Σi (subst_ty σA <$> σB) ≡
+                 interp_list (interp_list Σi σA) σB).
+    { rewrite /interp_list -list_fmap_compose.
+      apply list_fmap_equiv_ext_elem_of => ty0 hin0 /= w.
+      rewrite -interp_type_subst //.
+      apply extends_using_wf in hext => //.
+      destruct hext as (adef & ? & hF & _).
+      rewrite Forall_forall in hF.
+      inv hwfA; simplify_eq.
+      rewrite H3; by apply hF.
     }
-    rewrite /interp_fields.
-    iDestruct "hsem" as "[%hdom hfields]".
-    inv hwfB.
-    iExists ℓ, t, def, (subst_ty σ <$> σB), σt, fields, ifields.
-    iSplit.
-    { iPureIntro; split; first done.
-      split.
-      { by eapply inherits_using_trans; last by econstructor. }
-      split; first done.
-      split; first done.
-      split; first done.
-      split; last done.
-      assert (hwfB: wf_ty (ClassT B σB)).
-      { apply extends_using_wf in hext => //.
-        by repeat destruct hext as [? hext].
-      }
-      rewrite map_subst_ty_subst; last first.
-      { apply inherits_using_wf in hin => //.
-        destruct hin as (? & ? & ? & h); inv h; simplify_eq.
-        by rewrite H7.
-      }
-      assert (hadef' := hadef).
-      apply hmono in hadef'.
-      rewrite /wf_cdef_mono in hadef'.
-      clear hdom.
-      inv hext; simplify_eq.
-      rewrite H0 in hadef'.
-      apply subtype_targs_lift with (vs := adef.(generics)) => //.
-      - by apply wf_ty_class_inv in hwfB.
-      - by apply wf_ty_subst_map.
-      - move => i wi ti hwi hti hc.
-        inv hadef'; simplify_eq.
-        by apply (H7 i wi).
-      - move => i wi ti hwi hti hc.
-        inv hadef'; simplify_eq.
-        by apply (H8 i wi).
-    }
-    iSplit; last done.
-    iSplit; first by iPureIntro.
-    iIntros (f vis ty orig) "%hf".
-    by iApply "hfields".
+    rewrite (interp_tag_equivI _ _ hΣ).
+    inv hwfA.
+    iApply tag_extends_using_is_inclusion => //.
+    by rewrite /interp_list fmap_length.
   Qed.
 
-  Definition interp_variance v ty0 ty1 : iProp Σ :=
-    match v with
-    | Invariant => ∀ w,
-        interp_type_pre interp_type ty0 w ∗-∗ interp_type_pre interp_type ty1 w
-    | Covariant => ∀ w,
-        interp_type_pre interp_type ty0 w -∗ interp_type_pre interp_type ty1 w
-    | Contravariant => ∀ w,
-        interp_type_pre interp_type ty1 w -∗ interp_type_pre interp_type ty0 w
-    end.
-
-  Fixpoint iForall3 {A B C : Type} (P : A → B → C → iProp Σ)
-    (As : list A) (Bs: list B) (Cs : list C) {struct As}  : iProp Σ :=
-    match As, Bs, Cs with
-    | [], [], [] => True%I
-    | A :: As, B :: Bs, C :: Cs => (P A B C ∗ iForall3 P As Bs Cs)%I
-    | _, _, _ => False%I
-    end.
-
-  Definition interp_env_as_mixed :=
+  Definition interp_env_as_mixed (Σi: list (interp Σ)) :=
     ∀ i (ϕi: interp Σ),  Σi !! i = Some ϕi → ∀ v,  ϕi v -∗ interp_mixed interp_type v.
 
-  Definition Σinterp :=
+  Definition Σinterp (Σi: list (interp Σ)) (Σc : list constraint) :=
     ∀ i c, Σc !! i = Some c →
-    ∀ v, interp_type_pre interp_type c.1 v -∗ interp_type_pre interp_type c.2 v.
+    ∀ v, interp_type_pre interp_type c.1 Σi v -∗ interp_type_pre interp_type c.2 Σi v.
 
-  Definition interp_local_tys
-    (lty : local_tys) (le : local_env) : iProp Σ :=
-    interp_class_strict lty.(type_of_this).1 lty.(type_of_this).2 interp_type (LocV le.(vthis)) ∗
-    (∀ v ty, ⌜lty.(ctxt) !! v = Some ty⌝ -∗
-    ∃ val, ⌜le.(lenv) !! v = Some val⌝ ∗ interp_type ty val)%I.
+  Section Inclusion.
+    Hypothesis Σc: list constraint.
+    Hypothesis wfΣc: Forall wf_constraint Σc.
+    Hypothesis wf_parent : map_Forall (λ _cname, wf_cdef_parent Δ) Δ.
+    Hypothesis wf_mono : map_Forall (λ _ : string, wf_cdef_mono) Δ.
 
-  Section inclusion.
-    Hypothesis Σcoherency : Σinterp.
+  (* Extracting subproofs for clarity *)
+  Lemma subvariance_is_inclusion_aux Σi:
+    interp_env_as_mixed Σi →
+    Σinterp Σi Σc →
+    ∀ A adef σ0 σ1 v,
+    Δ !! A = Some adef →
+    wf_ty (ClassT A σ0) →
+    Forall wf_ty σ1 →
+    ⊢ □ iForall3 interp_variance adef.(generics) (interp_list Σi σ0) (interp_list Σi σ1) →
+    interp_type (ClassT A σ0) Σi v -∗
+    interp_type (ClassT A σ1) Σi v.
+  Proof.
+    move => ?? A adef σ0 σ1 v hadef hwfA hwfσ1.
+    iIntros "#hσ #h".
+    rewrite !interp_class_unfold !interp_tag_unseal /interp_tag_def /interp_fun !interp_car_simpl.
+    iDestruct "h" as (l t adef' σtA Σt fields ifields h) "[#hinst [hdyn hl]]".
+    destruct h as (-> & hadef' & hinherits & hfields & hdom); simplify_eq.
+    iExists l, t, adef, σtA, Σt, fields, ifields.
+    iSplit; first by iPureIntro.
+    iSplit; last by iSplit.
+    iClear "hdyn hl".
+    iModIntro; iNext.
+    iIntros (k v i0 i1 hv) "h0 h1".
+    rewrite !list_lookup_fmap.
+    destruct (σtA !! k) as [ta | ] eqn:hta; last first.
+    { by rewrite !option_equivI /=. }
+    destruct (σ0 !! k) as [t0 | ] eqn:ht0; last first.
+    { apply inherits_using_wf in hinherits => //.
+      destruct hinherits as (? & ? & ? & hwfA2).
+      inv hwfA; inv hwfA2; simplify_eq.
+      apply lookup_ge_None_1 in ht0.
+      apply lookup_lt_Some in hv.
+      by lia.
+    }
+    destruct (σ1 !! k) as [t1 | ] eqn:ht1; last first.
+    { by rewrite !option_equivI /=. }
+    iAssert (□ iForall3 interp_variance (neg_variance <$> adef.(generics)) (interp_list Σi σ1) (interp_list Σi σ0))%I as "#hσ2".
+    { iModIntro. by iApply neg_interp_variance. }
+    iSpecialize ("hinst" $! k v (interp_type ta Σt) (interp_type t0 Σi) hv).
+    iDestruct (iForall3_forall_1 with "hσ") as "hvar".
+    iDestruct (iForall3_forall_1 with "hσ2") as "hvar2".
+    iClear "hσ hσ2".
+    iSpecialize ("hvar" $! k v (interp_type t0 Σi) (interp_type t1 Σi) hv).
+    iSpecialize ("hvar2" $! k (neg_variance v) (interp_type t1 Σi) (interp_type t0 Σi)).
+    rewrite !list_lookup_fmap hta ht0 ht1 /= !option_equivI.
+    rewrite /interp_variance; destruct v => /=.
+    - iIntros (w).
+      iRewrite -"h0".
+      iRewrite -"h1".
+      iSplit; iIntros "#?".
+      + iApply "hvar" => //.
+        by iApply "hinst".
+      + iApply "hinst" => //.
+        by iApply "hvar".
+    - iIntros (w).
+      iRewrite -"h0".
+      iRewrite -"h1".
+      iIntros "#?".
+      iApply "hvar" => //.
+      by iApply "hinst".
+    - iIntros (w).
+      iRewrite -"h0".
+      iRewrite -"h1".
+      iIntros "#?".
+      iApply "hinst" => //.
+      by iApply "hvar".
+  Qed.
 
-    Hypothesis wfΣc : Forall wf_constraint Σc.
-
-    Hypothesis wfΣi : interp_env_as_mixed.
-
-    (* Main meat for A <: B → [|A|] ⊆ [|B|] *)
-    Theorem subtype_is_inclusion_aux A B:
-      map_Forall (λ _cname, wf_cdef_fields) Δ →
-      map_Forall (λ _cname, wf_cdef_fields_bounded) Δ →
-      map_Forall (λ _cname, wf_cdef_parent Δ) Δ →
-      map_Forall (λ _cname, wf_cdef_mono) Δ →
-      Σc ⊢ A <: B →
-      ∀ v,
-      wf_ty A →
-      interp_type_pre interp_type A v -∗
-      interp_type_pre interp_type B v
-      with subtype_targs_is_inclusion_aux Vs As Bs:
-      map_Forall (λ _cname, wf_cdef_fields) Δ →
-      map_Forall (λ _cname, wf_cdef_fields_bounded) Δ →
-      map_Forall (λ _cname, wf_cdef_parent Δ) Δ →
-      map_Forall (λ _cname, wf_cdef_mono) Δ →
-      Forall wf_ty As →
-      Forall wf_ty Bs →
-      Σc ⊢ As <:Vs:> Bs →
-      ⊢ iForall3 interp_variance Vs As Bs.
-    Proof.
-      { move => ????.
-        destruct 1 as [A | A h | A σA B σB adef hΔ hlen hext
-        | A adef hadef hL | A def σ0 σ1 hΔ hwfσ σ | | | | A | A B h
-        | A B h | A B C h0 h1 | A B | A B | A B C h0 h1
-        | A | A B C h0 h1 | A B hin] => v hwfA.
-        - rewrite /interp_mixed.
-          clear subtype_is_inclusion_aux subtype_targs_is_inclusion_aux.
-          elim: A v hwfA => //.
-          + move => v _; iIntros "h"; by repeat iLeft.
-          + move => v _; iIntros "h"; by iLeft; iRight; iLeft.
-          + move => v _; by rewrite /interp_nothing; iIntros "h".
-          + move => cname targs ? v hwf.
-            iIntros "h".
-            iLeft; iRight; iRight.
-            iExists cname, targs.
-            iSplitR; last done.
-            by iPureIntro.
-          + move => v _; iIntros "h"; by iRight.
-          + move => v _; by iIntros "h"; iLeft.
-          + move => s t hs ht v hwf.
-            inv hwf.
-            rewrite /interp_union.
-            iIntros "h".
-            iDestruct "h" as "[ h | h ]"; first by iApply hs.
-            by iApply ht.
-          + move => s t hs ht v hwf.
-            inv hwf.
-            rewrite /interp_inter.
-            iIntros "h".
-            iDestruct "h" as "[? _]"; by iApply hs.
-          + move => n v _.
-            rewrite /interp_generic.
-            iIntros "hv".
-            destruct (decide (n < length Σi)) as [hlt | hge].
-            * apply lookup_lt_is_Some_2 in hlt as [ϕ hϕ].
-              iApply wfΣi; last done.
-              by rewrite /= /interp_generic hϕ /=.
-            * rewrite /= /interp_generic lookup_ge_None_2 /=; last by apply not_lt.
-              done.
-          + move => cname v _;
-            rewrite /interp_ex.
-            iIntros "hv".
-            iDestruct "hv" as (targs) "hv".
-            iLeft; iRight; iRight.
-            by iExists _, _.
-        - clear subtype_is_inclusion_aux subtype_targs_is_inclusion_aux.
-          rewrite /=.
-          by iIntros "H".
-        - clear subtype_is_inclusion_aux subtype_targs_is_inclusion_aux.
-          apply wf_ty_class_inv in hwfA.
-          rewrite -!interp_type_unfold; by iApply extends_using_is_inclusion.
-        - clear subtype_is_inclusion_aux subtype_targs_is_inclusion_aux.
-          simpl.
-          iIntros "h".
-          iDestruct "h" as (σc hσc l t cdef σ σt fields ifields hpure) "[h hl]".
-          repeat destruct hpure as [? hpure]; simplify_eq.
-          iExists l, t, adef, σ, σt , fields, ifields; iSplit; last by iSplit.
-          iPureIntro.
-          repeat split => //.
-          inv hσc; simplify_eq.
-          replace [] with σc => //.
-          apply nil_length_inv.
-          by rewrite -hL.
-        - clear subtype_is_inclusion_aux subtype_targs_is_inclusion_aux.
-          iIntros "h".
-          iDestruct "h" as (l t adef Σin σt fields ifields) "[%hpure [#hifields #hl]]".
-          destruct hpure as (-> & hin & hwft & hokt & hadef & hsub & hfields).
-          iExists l, t, adef, Σin, σt, fields, ifields.
-          iSplitR; last by iSplit.
-          iPureIntro.
-          repeat split => //.
-          simplify_eq.
-          by eapply subtype_targs_trans.
-        - clear subtype_is_inclusion_aux subtype_targs_is_inclusion_aux.
-          by rewrite /= /interp_mixed.
-        - clear subtype_is_inclusion_aux subtype_targs_is_inclusion_aux.
-          iIntros "h"; by iLeft.
-        - clear subtype_is_inclusion_aux subtype_targs_is_inclusion_aux.
-          iIntros "h"; by iRight; iLeft.
-        - clear subtype_is_inclusion_aux subtype_targs_is_inclusion_aux.
-          iIntros "H".
-          iRight; iRight.
-          iExists A, targs.
-          iSplitR; last done.
-          by iPureIntro.
-        - clear subtype_is_inclusion_aux subtype_targs_is_inclusion_aux.
-          by iIntros "h"; iLeft.
-        - clear subtype_is_inclusion_aux subtype_targs_is_inclusion_aux.
-          by iIntros "h"; iRight.
-        - rewrite /interp_union.
-          iIntros "[h | h]".
-          + iApply subtype_is_inclusion_aux; [done | done | done | done | exact h0 | | ].
-            * inv hwfA; by assumption.
-            * by iAssumption.
-          + iApply subtype_is_inclusion_aux; [done | done | done | done | exact h1 | | ].
-            * inv hwfA; by assumption.
-            * by iAssumption.
-        - clear subtype_is_inclusion_aux subtype_targs_is_inclusion_aux.
-          iIntros "[h _]".
-          by iAssumption.
-        - clear subtype_is_inclusion_aux subtype_targs_is_inclusion_aux.
-          iIntros "[_ ?]".
-          by iAssumption.
-        - iIntros "h".
-          iSplit.
-          + iApply subtype_is_inclusion_aux; [done | done | done | done | exact h0 | done | ].
-            by iAssumption.
-          + iApply subtype_is_inclusion_aux; [done | done | done | done | exact h1 | done | ].
-            by iAssumption.
-        - done.
-        - iIntros "h".
-          iApply subtype_is_inclusion_aux; [done | done | done | done | exact h1 | | ].
-          + apply subtype_wf in h0; [ | done | done | done ].
-            by assumption.
-          + iApply subtype_is_inclusion_aux; [done | done | done | done | exact h0 | done | ].
-            by iAssumption.
-        - apply elem_of_list_lookup_1 in hin as [i hin].
-          by apply Σcoherency in hin.
+  Lemma submixed_is_inclusion_aux Σi:
+    interp_env_as_mixed Σi →
+    Σinterp Σi Σc →
+    ∀ A v, wf_ty A →
+    interp_type A Σi v -∗
+    interp_type MixedT Σi v.
+  Proof.
+    move => wfΣi ? A v.
+    rewrite !interp_type_unfold /=.
+    elim: A v.
+    - move => v _; iIntros "h"; by repeat iLeft.
+    - move => v _; iIntros "h"; by iLeft; iRight; iLeft.
+    - move => v _; by rewrite /interp_nothing; iIntros "h".
+    - done.
+    - move => cname targs ? v hwf.
+      iIntros "h".
+      iLeft; iRight; iRight.
+      iExists cname.
+      iExists (interp_list Σi targs).
+      rewrite /= !interp_tag_unseal /interp_tag_def.
+      rewrite /interp_fun !interp_car_simpl.
+      iDestruct "h" as (l t cdef σ Σt fields ifields h) "[#hinst [hdyn hloc]]".
+      destruct h as (-> & hcdef & ? & ? & ?).
+      iExists cdef; iSplitR.
+      { iPureIntro; split => //.
+        rewrite fmap_length.
+        inv hwf; by simplify_eq.
       }
-      move => ???? hwfA hwfB.
-      destruct 1 as [ | ????? h0 h1 h | ????? h0 h | ????? h0 h].
-      - clear subtype_is_inclusion_aux subtype_targs_is_inclusion_aux.
+      iExists l, t, cdef, σ, Σt, fields, ifields.
+      iSplitR; first done.
+      iSplit; last by iSplit.
+      iClear "hdyn hloc".
+      iModIntro; iNext.
+      iIntros (k v i0 i1 hv) "#h0 #h1".
+      iApply "hinst" => //.
+      destruct (targs !! k) as [ty | ] eqn:hty; last first.
+      { by rewrite !list_lookup_fmap hty !option_equivI /=. }
+      rewrite /interp_list !list_lookup_fmap hty !option_equivI /=.
+      iRewrite -"h1".
+      iPureIntro.
+      move => x.
+      by rewrite interp_type_unfold.
+    - move => v _; iIntros "h"; by iRight.
+    - move => v _; by iIntros "h"; iLeft.
+    - move => s t hs ht v hwf.
+      inv hwf.
+      rewrite /interp_union.
+      iIntros "h".
+      iDestruct "h" as "[ h | h ]"; first by iApply hs.
+      by iApply ht.
+    - move => s t hs ht v hwf.
+      inv hwf.
+      rewrite /interp_inter.
+      iIntros "h".
+      iDestruct "h" as "[? _]"; by iApply hs.
+    - move => n v _.
+      rewrite /interp_generic.
+      iIntros "hv".
+      destruct (decide (n < length Σi)) as [hlt | hge].
+      + apply lookup_lt_is_Some_2 in hlt as [ϕ hϕ].
+        iApply wfΣi; last done.
+        by rewrite /= /interp_generic hϕ /=.
+      + rewrite /= /interp_generic lookup_ge_None_2 /=; last by apply not_lt.
         done.
-      - simpl.
-        apply Forall_cons_1 in hwfA as [hA hwfA].
-        apply Forall_cons_1 in hwfB as [hB hwfB].
-        iSplitR.
-        + iIntros (w); iSplit.
-          * by iApply subtype_is_inclusion_aux.
-          * by iApply subtype_is_inclusion_aux.
-        + by iApply subtype_targs_is_inclusion_aux.
-      - simpl.
-        apply Forall_cons_1 in hwfA as [hA hwfA].
-        apply Forall_cons_1 in hwfB as [hB hwfB].
-        iSplitR.
-        + iIntros (w).
-          by iApply subtype_is_inclusion_aux.
-        + by iApply subtype_targs_is_inclusion_aux.
-      - simpl.
-        apply Forall_cons_1 in hwfA as [hA hwfA].
-        apply Forall_cons_1 in hwfB as [hB hwfB].
-        iSplitR.
-        + iIntros (w).
-          by iApply subtype_is_inclusion_aux.
-        + by iApply subtype_targs_is_inclusion_aux.
-    Qed.
+    - move => cname v _;
+      rewrite /interp_ex.
+      iIntros "hv".
+      iDestruct "hv" as (targs) "hv".
+      iLeft; iRight; iRight.
+      by iExists _, _.
+  Qed.
 
-    (* A <: B → [|A|] ⊆ [|B|] *)
-    Theorem subtype_is_inclusion:
-      map_Forall (λ _cname, wf_cdef_fields) Δ →
-      map_Forall (λ _cname, wf_cdef_fields_bounded) Δ →
-      map_Forall (λ _cname, wf_cdef_parent Δ) Δ →
-      map_Forall (λ _cname, wf_cdef_mono) Δ →
-      ∀ A B, Σc ⊢ A <: B →
-      ∀ v,
-      wf_ty A →
-      interp_type A v -∗ interp_type B v.
-    Proof.
-      move => ???? A B hAB v ?.
+  (* Main meat for A <: B → [|A|] ⊆ [|B|] *)
+  Theorem subtype_is_inclusion_aux Σi A B:
+    interp_env_as_mixed Σi →
+    Σinterp Σi Σc →
+    Σc ⊢ A <: B →
+    ∀ v,
+    wf_ty A →
+    interp_type_pre interp_type A Σi v -∗
+    interp_type_pre interp_type B Σi v
+    with subtype_targs_is_inclusion_aux Σi Vs As Bs:
+    interp_env_as_mixed Σi →
+    Σinterp Σi Σc →
+    Forall wf_ty As →
+    Forall wf_ty Bs →
+    Σc ⊢ As <:Vs:> Bs →
+    ⊢ □ iForall3 interp_variance Vs (interp_list Σi As) (interp_list Σi Bs).
+  Proof.
+    { move => wfΣi Σcoherency.
+      destruct 1 as [A | A h | A σA B σB adef hΔ hlen hext
+      | A adef hadef hL | A def σ0 σ1 hΔ hwfσ hσ | | | | A | A B h
+      | A B h | A B C h0 h1 | A B | A B | A B C h0 h1
+      | A | A B C h0 h1 | A B hin] => v hwfA.
+      - clear subtype_is_inclusion_aux subtype_targs_is_inclusion_aux.
+        rewrite -!interp_type_unfold.
+        by eapply submixed_is_inclusion_aux.
+      - clear subtype_is_inclusion_aux subtype_targs_is_inclusion_aux.
+        rewrite /=.
+        by iIntros "H".
+      - clear subtype_is_inclusion_aux subtype_targs_is_inclusion_aux.
+        rewrite -!interp_type_unfold; by iApply extends_using_is_inclusion.
+      - clear subtype_is_inclusion_aux subtype_targs_is_inclusion_aux.
+        simpl.
+        iIntros "h".
+        iDestruct "h" as (Σt cdef h) "h".
+        destruct h as (hadef' & hLt); simplify_eq.
+        replace Σt with (@nil (interp Σ)) => //.
+        rewrite hL in hLt.
+        apply nil_length_inv in hLt.
+        by rewrite hLt.
+      - apply subtype_targs_is_inclusion_aux with (Σi := Σi) in hσ => //; last first.
+        { by apply wf_ty_class_inv in hwfA. }
+        clear subtype_is_inclusion_aux subtype_targs_is_inclusion_aux.
+        rewrite -!interp_type_unfold.
+        by iApply subvariance_is_inclusion_aux.
+      - clear subtype_is_inclusion_aux subtype_targs_is_inclusion_aux.
+        by rewrite /= /interp_mixed.
+      - clear subtype_is_inclusion_aux subtype_targs_is_inclusion_aux.
+        iIntros "h"; by iLeft.
+      - clear subtype_is_inclusion_aux subtype_targs_is_inclusion_aux.
+        iIntros "h"; by iRight; iLeft.
+      - clear subtype_is_inclusion_aux subtype_targs_is_inclusion_aux.
+        iIntros "H".
+        iRight; iRight.
+        iExists A, (interp_list Σi targs).
+        inv hwfA.
+        iExists def; iSplitR.
+        + by rewrite fmap_length.
+        + by rewrite -interp_type_unfold -interp_class_unfold.
+      - clear subtype_is_inclusion_aux subtype_targs_is_inclusion_aux.
+        by iIntros "h"; iLeft.
+      - clear subtype_is_inclusion_aux subtype_targs_is_inclusion_aux.
+        by iIntros "h"; iRight.
+      - clear subtype_targs_is_inclusion_aux.
+        rewrite /= /interp_union. iIntros "[h | h]".
+        + iApply subtype_is_inclusion_aux; [done | done | exact h0 | | ].
+          * inv hwfA; by assumption.
+          * by iAssumption.
+        + iApply subtype_is_inclusion_aux; [done | done | exact h1 | | ].
+          * inv hwfA; by assumption.
+          * by iAssumption.
+      - clear subtype_is_inclusion_aux subtype_targs_is_inclusion_aux.
+        iIntros "[h _]".
+        by iAssumption.
+      - clear subtype_is_inclusion_aux subtype_targs_is_inclusion_aux.
+        iIntros "[_ ?]".
+        by iAssumption.
+      - clear subtype_targs_is_inclusion_aux.
+        rewrite /= /interp_inter.
+        iIntros "h".
+        iSplit.
+        + iApply subtype_is_inclusion_aux; [done | done | exact h0 | done | ].
+          by iAssumption.
+        + iApply subtype_is_inclusion_aux; [done | done | exact h1 | done | ].
+          by iAssumption.
+      - done.
+      - iIntros "h".
+        iApply subtype_is_inclusion_aux; [done | done | exact h1 | | ].
+        + apply subtype_wf in h0; [ | done | done | done ].
+          by assumption.
+        + iApply subtype_is_inclusion_aux; [done | done | exact h0 | done | ].
+          by iAssumption.
+      - apply elem_of_list_lookup_1 in hin as [i hin].
+        by apply Σcoherency in hin.
+    }
+    move => wfΣi ? hwfA hwfB.
+    destruct 1 as [ | ????? h0 h1 h | ????? h0 h | ????? h0 h].
+    - clear subtype_is_inclusion_aux subtype_targs_is_inclusion_aux.
+      by iStartProof.
+    - simpl.
+      apply Forall_cons_1 in hwfA as [hA hwfA].
+      apply Forall_cons_1 in hwfB as [hB hwfB].
+      iSplitR.
+      + iIntros (w); iModIntro; iSplit.
+        * rewrite !interp_type_unfold.
+          by iApply subtype_is_inclusion_aux.
+        * rewrite !interp_type_unfold.
+          by iApply subtype_is_inclusion_aux.
+      + by iApply subtype_targs_is_inclusion_aux.
+    - simpl.
+      apply Forall_cons_1 in hwfA as [hA hwfA].
+      apply Forall_cons_1 in hwfB as [hB hwfB].
+      iSplitR.
+      + iIntros (w); iModIntro.
+        rewrite !interp_type_unfold.
+        by iApply subtype_is_inclusion_aux.
+      + by iApply subtype_targs_is_inclusion_aux.
+    - simpl.
+      apply Forall_cons_1 in hwfA as [hA hwfA].
+      apply Forall_cons_1 in hwfB as [hB hwfB].
+      iSplitR.
+      + iIntros (w); iModIntro.
+        rewrite !interp_type_unfold.
+        by iApply subtype_is_inclusion_aux.
+      + by iApply subtype_targs_is_inclusion_aux.
+  Qed.
+
+  (* A <: B → [|A|] ⊆ [|B|] *)
+  Theorem subtype_is_inclusion Σi:
+    interp_env_as_mixed Σi →
+    Σinterp Σi Σc →
+    ∀ A B, Σc ⊢ A <: B →
+    ∀ v,
+    wf_ty A →
+    interp_type A Σi v -∗ interp_type B Σi v.
+  Proof.
+    move => ?? A B hAB v ?.
     rewrite !interp_type_unfold.
     by iApply subtype_is_inclusion_aux.
-    Qed.
+  Qed.
 
-    Lemma interp_local_tys_is_inclusion lty rty le:
-      map_Forall (λ _cname, wf_cdef_fields) Δ →
-      map_Forall (λ _cname, wf_cdef_fields_bounded) Δ →
-      map_Forall (λ _cname, wf_cdef_parent Δ) Δ →
-      map_Forall (λ _ : string, wf_cdef_mono) Δ →
-      wf_lty lty →
-      Forall (λ (i: interp Σ), ∀ v, Persistent (i v)) Σi →
-      Σc ⊢ lty <:< rty →
-      interp_local_tys lty le -∗
-      interp_local_tys rty le.
-    Proof.
-      move => ???? hlty hpers hsub; iIntros "[#Hthis Hle]".
-      destruct hsub as [hthis hsub].
-      assert (hthis2: type_of_this lty = type_of_this rty).
-      { rewrite /this_type in hthis.
-        rewrite (surjective_pairing (type_of_this lty))
-        (surjective_pairing (type_of_this rty)).
-        by case : hthis => -> ->.
-      }
-      rewrite hthis2.
-      iSplitR; first done.
-      iIntros (v ty) "%Hv".
-      apply hsub in Hv as (B & hB & hsubB).
-      iDestruct ("Hle" $! v B hB) as (val) "[%Hv' #H]".
-      iExists val; iSplitR; first done.
-      iApply subtype_is_inclusion => //.
-      by apply hlty in hB.
-    Qed.
-  End inclusion.
+  Definition interp_this_def
+    (C: tag)
+    (Σi : list (interp Σ))
+    : interp Σ :=
+    Interp (
+      λ (w : value), (∃ ℓ t σ (Σt: list (interp Σ))
+       (fields: stringmap ((visibility * lang_ty) * tag))
+       (ifields: gmapO string (laterO (sem_typeO Σ))),
+      ⌜w = LocV ℓ ∧
+       inherits_using t C σ ∧
+       has_fields t fields ∧
+       dom fields = dom ifields⌝ ∗
+
+       □ ▷ (∀ k i0 i1,
+         ((λ ty, interp_type ty Σt) <$> σ) !! k ≡ Some i0 →
+         Σi !! k ≡ Some i1 →
+         i0 ≡ i1) ∗
+
+      (∀ f vis ty orig, ⌜has_field f t vis ty orig⌝ -∗
+        ifields !! f ≡ Some (Next (interp_car (interp_type ty Σt)))) ∗
+
+      (ℓ ↦ (t, ifields)))%I
+    ).
+
+   Local Definition interp_this_aux
+     (C: tag) (Σi : list (interp Σ)) : seal (@interp_this_def C Σi).
+   Proof. by eexists. Qed.
+
+  Definition interp_this C Σi : interp Σ := (interp_this_aux C Σi).(unseal).
+
+   Definition interp_this_unseal 
+     (C: tag)
+     (Σi : list (interp Σ))
+     : interp_this C Σi = interp_this_def C Σi :=
+     (interp_this_aux C Σi).(seal_eq).
+
+  Definition interp_this_type C (σC: list lang_ty) Σi : interp Σ :=
+    interp_this C (interp_list Σi σC).
+
+  Definition interp_local_tys Σi
+    (lty : local_tys) (le : local_env) : iProp Σ := 
+    interp_this_type lty.(type_of_this).1 lty.(type_of_this).2 Σi (LocV le.(vthis)) ∗
+    (∀ v ty, ⌜lty.(ctxt) !! v = Some ty⌝ -∗
+    ∃ val, ⌜le.(lenv) !! v = Some val⌝ ∗ interp_type ty Σi val)%I.
+
+  Lemma interp_local_tys_is_inclusion Σi lty rty le:
+    interp_env_as_mixed Σi →
+    Σinterp Σi Σc →
+    wf_lty lty →
+    Forall (λ (i: interp Σ), ∀ v, Persistent (i v)) Σi →
+    Σc ⊢ lty <:< rty →
+    interp_local_tys Σi lty le -∗
+    interp_local_tys Σi rty le.
+  Proof.
+    move => ?? hlty hpers hsub; iIntros "[#Hthis Hle]".
+    destruct hsub as [hthis hsub].
+    assert (hthis2: type_of_this lty = type_of_this rty).
+    { rewrite /this_type in hthis.
+      rewrite (surjective_pairing (type_of_this lty))
+      (surjective_pairing (type_of_this rty)).
+      by case : hthis => -> ->.
+    }
+    rewrite /this_type hthis2.
+    iSplitR; first done.
+    iIntros (v ty) "%Hv".
+    apply hsub in Hv as (B & hB & hsubB).
+    iDestruct ("Hle" $! v B hB) as (val) "[%Hv' #H]".
+    iExists val; iSplitR; first done.
+    iApply subtype_is_inclusion => //.
+    by apply hlty in hB.
+  Qed.
 
   (* Specialized version for existential types. Will help during the
    * proof of adequacy for runtime checks.
    *)
-  Theorem inherits_is_ex_inclusion:
-    map_Forall (λ _cname, wf_cdef_fields) Δ →
-    map_Forall (λ _cname, wf_cdef_fields_bounded) Δ →
-    map_Forall (λ _cname, wf_cdef_parent Δ) Δ →
-    map_Forall (λ _cname, wf_cdef_mono) Δ →
+  Theorem inherits_is_ex_inclusion Σi:
     ∀ A B, inherits A B →
-    ∀ v, interp_type (ExT A) v -∗ interp_type (ExT B) v.
+    ∀ v, interp_type (ExT A) Σi v -∗ interp_type (ExT B) Σi v.
   Proof.
-    move => ?? hp ?.
     induction 1 as [ x | x y z hxy hyz hi ] => // v.
     rewrite interp_ex_unfold.
     iIntros "H".
     iApply hi; clear hyz hi.
-    iDestruct "H" as (σx) "[%hσx H]".
-    destruct hxy as [x y xdef σy hxdef hsuper].
+    iDestruct "H" as (Σx xdef h) "H".
+    destruct h as [hxdef hlen].
+    destruct hxy as [x y xdef' σy hxdef' hsuper]; simplify_eq.
     assert (hext: extends_using x y σy) by (econstructor; by eauto).
-    assert (hydef : is_Some (Δ !! y)).
-    { apply hp in hxdef.
-      rewrite /wf_cdef_parent hsuper in hxdef.
-      destruct hxdef as [h _]; inv h; by simplify_eq.
-    }
-    destruct hydef as [ydef hydef].
-    iAssert (interp_type (ClassT y (subst_ty σx <$> σy)) v) with "[H]" as "Hext".
-    { iApply extends_using_is_inclusion => //.
-      - by apply wf_ty_class_inv in hσx.
-      - by rewrite interp_class_unfold.
-    }
-    rewrite interp_class_unfold interp_ex_unfold.
-    iExists (subst_ty σx <$> σy); iSplitR; last done.
+    iDestruct ((tag_extends_using_is_inclusion wf_parent wf_mono x y σy) with "H") as "H" => //.
+    rewrite interp_ex_unfold /interp_ex /=.
+    apply wf_parent in hxdef'.
+    rewrite /wf_cdef_parent hsuper in hxdef'.
+    destruct hxdef' as [hwf _].
+    inv hwf.
+    iExists _, def; iSplitR; last done.
     iPureIntro.
-    apply wf_ty_class with ydef => //.
-    { rewrite map_length.
-      apply hp in hxdef.
-      rewrite /wf_cdef_parent hsuper in hxdef.
-      destruct hxdef as [h _]; inv h; by simplify_eq.
-    }
-    apply wf_ty_subst_map; first by apply wf_ty_class_inv in hσx.
-    apply hp in hxdef.
-    rewrite /wf_cdef_parent hsuper in hxdef.
-    destruct hxdef as [h _].
-    by apply wf_ty_class_inv in h.
+    split => //.
+    by rewrite fmap_length.
   Qed.
-
-  (* Helper to lift the conclusions of interp_class into a super class *)
-  Lemma interp_fields_inclusion t σt fields ifields σ C rec:
-    wf_no_cycle Δ →
-    map_Forall (λ _cname, wf_cdef_parent Δ) Δ →
-    map_Forall (λ _cname, wf_cdef_fields) Δ →
-    map_Forall (λ _cname, wf_cdef_fields_bounded) Δ →
-    inherits_using t C σ →
-    interp_fields t σt fields ifields rec -∗
-    interp_fields C (subst_ty σt <$> σ) fields ifields rec.
-  Proof.
-    move => ??? hb hin.
-    rewrite /interp_fields.
-    iIntros "[%hdom #hfields]".
-    iSplit; first done.
-    iIntros (f vis ty orig) "%hf".
-    assert (hfC: has_field f t vis (subst_ty σ ty) orig) by (by eapply has_field_inherits_using).
-    iSpecialize ("hfields" $! f vis (subst_ty σ ty) orig hfC).
-    rewrite subst_ty_subst //.
-    apply has_field_bounded in hf => //.
-    destruct hf as (def & hdef & hfty).
-    apply inherits_using_wf in hin => //.
-    destruct hin as (? & ? & ? & hwf).
-    inv hwf; simplify_eq.
-    by rewrite H4.
-  Qed.
-
+  End Inclusion.
 End proofs.
