theories/adequacy.v
@@ -41,21 +41,19 @@ Section proofs.
     ∃ (iFs : gmapO string (laterO (sem_typeO Σ))),
     sh !! ℓ ≡ Some (t, iFs) ∗ heap_models_fields iFs vs.
 
-  Lemma expr_adequacy Σc Σi e lty le ty val :
-    map_Forall (λ _cname, wf_cdef_fields) Δ →
-    map_Forall (λ _cname, wf_cdef_fields_bounded) Δ →
-    map_Forall (λ _cname, wf_cdef_parent Δ) Δ →
-    map_Forall (λ _ : string, wf_cdef_mono) Δ →
-    Σinterp Σc Σi →
-    interp_env_as_mixed Σc Σi →
+  Lemma expr_adequacy (Σc: list constraint) (Σi: list (interp Σ)) e lty le ty val :
+    map_Forall (λ _, wf_cdef_parent Δ) Δ →
+    map_Forall (λ _, wf_cdef_mono) Δ →
+    Σinterp Σi Σc →
+    interp_env_as_mixed Σi →
     Forall wf_constraint Σc →
     wf_lty lty →
     expr_eval le e = Some val →
     expr_has_ty Σc lty e ty →
-    interp_local_tys Σc Σi  lty le -∗
-    interp_type Σc Σi ty val.
+    interp_local_tys Σi lty le -∗
+    interp_type ty Σi val.
   Proof.
-    move => ???????? he h; move: le val he.
+    move => ?????? he h; move: le val he.
     elim: h => [z | b | | op e1 e2 hop he1 hi1 he2 hi2 |
         op e1 e2 hop he1 hi1 he2 hi2 | e1 e2 h1 hi1 h2 hi2 | e0 h hi |
         v vty hv | | exp S T hS hi hwf hok hsub ] => le val he; iIntros "#Hlty".
@@ -126,18 +124,39 @@ Section proofs.
       rewrite H0 in H; by case: H => ->.
     - inv he.
       iDestruct "Hlty" as "[Hthis ?]".
-      rewrite /this_type interp_class_unfold.
-      by iApply interp_class_from_strict.
+      rewrite /interp_this_type interp_this_unseal /interp_this_def /=.
+      iDestruct "Hthis" as (??????) "[%H [#hinst [hdyn hloc]]]".
+      rewrite /this_type interp_class_unfold interp_tag_unseal /interp_tag_def /=.
+      destruct lty as [[this σthis] lty]; simpl in *.
+      destruct H as ([= <-] & hin & hfields & hdom).
+      assert (h0: is_Some (Δ !! this)).
+      { apply inherits_using_wf in hin => //.
+        destruct hin as (?&?&?&h).
+        by inv h.
+      }
+      destruct h0 as [thisdef hthisdef].
+      iExists _,_,_,_,_,_, _.
+      iSplit; first done.
+      iSplit; last by iSplit.
+      iModIntro; iNext.
+      iIntros (k v i0 i1 hv) "h0 h1".
+      iSpecialize ("hinst" $! k i0 i1).
+      rewrite !list_lookup_fmap.
+      iSpecialize ("hinst" with "h0 h1").
+      rewrite /interp_variance; destruct v; iIntros (w); iRewrite "hinst".
+      + by iSplit; iIntros.
+      + by iIntros.
+      + by iIntros.
     - apply hi in he.
       iApply subtype_is_inclusion => //.
       + by apply expr_has_ty_wf in hS.
       + by iApply he.
   Qed.
 
-  Lemma interp_local_tys_update Σc Σi v lty le ty val :
-    interp_local_tys Σc Σi lty le -∗
-    interp_type Σc Σi ty val -∗
-    interp_local_tys Σc Σi (<[v:=ty]>lty) (<[v:=val]>le).
+  Lemma interp_local_tys_update Σi v lty le ty val :
+    interp_local_tys Σi lty le -∗
+    interp_type ty Σi val -∗
+    interp_local_tys Σi (<[v:=ty]>lty) (<[v:=val]>le).
   Proof.
     iIntros "#[Hthis Hi] #?".
     iSplit; first done.
@@ -149,12 +168,10 @@ Section proofs.
   Qed.
 
   Lemma interp_local_tys_list Σc Σi lty le targs args vargs l t σ:
-    map_Forall (λ _cname, wf_cdef_fields) Δ →
-    map_Forall (λ _cname, wf_cdef_fields_bounded) Δ →
     map_Forall (λ _cname, wf_cdef_parent Δ) Δ →
     map_Forall (λ _ : string, wf_cdef_mono) Δ →
-    Σinterp Σc Σi →
-    interp_env_as_mixed Σc Σi →
+    Σinterp Σi Σc →
+    interp_env_as_mixed Σi →
     Forall wf_constraint Σc →
     wf_lty lty →
     dom targs = dom args →
@@ -163,12 +180,12 @@ Section proofs.
     targs !! x = Some ty →
     args !! x = Some arg →
     expr_has_ty Σc lty arg ty) →
-    interp_class_strict Σc t σ (interp_type Σc Σi) (LocV l) -∗
-    interp_local_tys Σc Σi lty le -∗
-    interp_local_tys Σc Σi {| type_of_this := (t, σ); ctxt := targs |}
-                           {| vthis := l; lenv := vargs |}.
+    interp_this_type t σ Σi (LocV l) -∗
+    interp_local_tys Σi lty le -∗
+    interp_local_tys Σi {| type_of_this := (t, σ); ctxt := targs |}
+                        {| vthis := l; lenv := vargs |}.
   Proof.
-    move => ???????? hdom hargs helt.
+    move => ?????? hdom hargs helt.
     iIntros "#Hl #[Hthis Hle]".
     iSplit; first done.
     iIntros (v ty) "%hin".
@@ -193,7 +210,7 @@ Section proofs.
     iApply expr_adequacy => //.
     by iSplit.
   Qed.
-
+  
   Lemma heap_models_update Σc Σi h l rt vs t σt f vis fty orig v:
     map_Forall (λ _cname, wf_cdef_parent Δ) Δ →
     map_Forall (λ _cname, wf_cdef_fields) Δ →
@@ -201,54 +218,134 @@ Section proofs.
     map_Forall (λ _ : string, wf_cdef_fields_wf) Δ →
     map_Forall (λ _cname, wf_field_mono) Δ →
     map_Forall (λ _ : string, wf_cdef_mono) Δ →
-    Σinterp Σc Σi →
-    interp_env_as_mixed Σc Σi →
+    Σinterp Σi Σc →
+    interp_env_as_mixed Σi →
     Forall wf_constraint Σc →
     h !! l = Some (rt, vs) →
     has_field f t vis fty orig →
     wf_ty (ClassT t σt) →
     match vis with
-    | Public => interp_type Σc Σi (ClassT t σt) (LocV l)
-    | Private => interp_class_strict Σc t σt (interp_type Σc Σi) (LocV l)
+    | Public => interp_type (ClassT t σt) Σi (LocV l)
+    | Private => interp_this_type t σt Σi (LocV l)
     end -∗
-    interp_type Σc Σi (subst_ty σt fty) v -∗
+    interp_type (subst_ty σt fty) Σi v -∗
     heap_models h -∗
     heap_models (<[l:=(rt, <[f:=v]> vs)]> h).
   Proof.
-    move => ???? hfb ???? hheap hfield hwf.
+    move => ????????? hheap hfield hwf.
     iIntros "hrecv".
-    iAssert (∃ t' def σ' σt' fields ifields,
-      ⌜inherits_using t' t σ' ∧
-       wf_ty (ClassT t' σt') ∧
-       Δ !! t = Some def ∧
-       match vis with
-       | Public => Σc ⊢ subst_ty σt' <$> σ' <: generics def :> σt
-       | Private => subst_ty σt' <$> σ' = σt
-       end ∧ has_fields t' fields⌝ ∗
-      interp_fields t' σt' (dom fields) ifields (interp_type Σc Σi) ∗
+    iAssert (∃ t' σ' Σt fields (ifields: gmapO string (laterO (sem_typeO Σ))),
+      ⌜inherits_using t' t σ' ∧ has_fields t' fields ∧ dom fields = dom ifields⌝ ∗
+       (□ ▷ ∀ w,
+           interp_type fty (interp_list Σi σt) w ∗-∗
+           interp_type (subst_ty σ' fty) Σt w)
+       ∗
+       (∀ f vis ty orig, ⌜has_field f t' vis ty orig⌝ -∗ ifields !! f ≡ Some (Next (interp_car (interp_type ty Σt)))) ∗
       l↦(t',ifields))%I with "[hrecv]" as "hrecv".
     { destruct vis.
-      - rewrite interp_class_unfold.
-        iDestruct "hrecv" as (l' t' def σ' σt' fields ifields) "[%H [hsem hl]]".
-        destruct H as ([= <-] & H).
-        repeat destruct H as [? H].
-        iExists _, _, _, _ ,_ ,_.
-        by repeat iSplit => //.
-      - iDestruct "hrecv" as (l' t' σ' σt' fields ifields) "[%H [hsem hl]]".
-        destruct H as ([= <-] & H).
-        repeat destruct H as [? H].
-        inv hwf.
-        iExists _, _, _ ,_ ,_, _.
-        by repeat iSplit => //.
+      - rewrite interp_class_unfold !interp_tag_unseal /interp_tag_def /interp_fun !interp_car_simpl.
+        iDestruct "hrecv" as (l' t' def σ' Σt fields ifields) "[%H [#hinst [hdyn hl]]]".
+        destruct H as ([= <-] & hdef & hinherits & hfields & hdom).
+        iExists t', σ', Σt, fields, ifields.
+        iSplitR; first done.
+        iSplitR; last by iSplit.
+        iModIntro; iNext; iIntros (w).
+        assert (hl0: length def.(generics) = length σ').
+        { apply inherits_using_wf in hinherits => //.
+          destruct hinherits as (? & ? & ? & hhh).
+          inv hhh; by simplify_eq.
+        }
+        assert (hl1: length σ' = length σt).
+        { apply inherits_using_wf in hinherits => //.
+          destruct hinherits as (? & ? & ? & hhh).
+          inv hhh; inv hwf; simplify_eq.
+          by rewrite H4 H7.
+        }
+        assert (hwf_fty: wf_ty fty).
+        { by apply has_field_wf in hfield. }
+        assert (hb: bounded (length σ') fty).
+        { apply has_field_bounded in hfield => //.
+          destruct hfield as (? & ? & hf); simplify_eq.
+          by rewrite -hl0.
+        }
+        apply has_field_mono in hfield => //.
+        destruct hfield as (def' & hdef' & [hco hcontra]); simplify_eq.
+        iAssert (□ iForall3 interp_variance def'.(generics) (interp_list Σt σ') (interp_list Σi σt))%I as "hf0".
+        { iModIntro.
+          move: hl0 hl1.
+          generalize (generics def') => ll.
+          clear.
+          move => hl0 hl1.
+          iInduction ll as [ | hd tl] "HI" forall (σt σ' hl0 hl1).
+          { by destruct σt; destruct σ'. }
+          destruct σt as [ | ty σt] => /=.
+          { by rewrite hl1 in hl0. }
+          destruct σ' as [ | t' σ'] => //=.
+          case: hl0 => hl0.
+          case: hl1 => hl1.
+          iSplitL; first by iApply ("hinst" $! 0).
+          iApply "HI" => //.
+          iModIntro; iIntros (k v i0 i1 hk) "#h0 #h1".
+          by iApply ("hinst" $! (S k)).
+        }
+        iAssert (□ iForall3 interp_variance (neg_variance <$> def'.(generics)) (interp_list Σi σt) (interp_list Σt σ'))%I as "hf1".
+        { by iModIntro; iApply neg_interp_variance. }
+        iClear "hinst".
+        iSplit; iIntros "#?".
+        + iAssert (interp_type (subst_ty σ' fty) Σt w) as "h"; last done.
+          rewrite interp_type_subst //.
+          by iApply (interp_with_mono with "hf1").
+        + iApply (interp_with_mono with "hf0") => //.
+          by rewrite -interp_type_subst.
+      - rewrite /interp_this_type interp_this_unseal /interp_this_def /=.
+        iDestruct "hrecv" as (l' t' σ' Σt fields ifields) "[%H [#hinst [hdyn hl]]]".
+        destruct H as ([= <-] & hinherits & hfields & hdom).
+        assert (hl1: length σ' = length σt).
+        { apply inherits_using_wf in hinherits => //.
+          destruct hinherits as (? & ? & ? & hhh).
+          inv hhh; inv hwf; simplify_eq.
+          by rewrite H4 H7.
+        }
+        assert (hb: bounded (length σ') fty).
+        { apply has_field_bounded in hfield => //.
+          destruct hfield as (? & ? & hf); simplify_eq.
+          apply inherits_using_wf in hinherits => //.
+          destruct hinherits as (? & ? & ? & hh).
+          inv hh; simplify_eq.
+          by rewrite H5.
+        }
+        iExists t', σ', Σt, fields, ifields.
+        iSplitR; first done.
+        iSplitR; last by iSplit.
+        iModIntro; iNext; iIntros (w).
+        rewrite interp_type_subst //.
+        iAssert (interp_list Σi σt ≡ interp_list Σt σ')%I as "hctxt".
+        { rewrite list_equivI; iIntros (k).
+          iSpecialize ("hinst" $! k).
+          rewrite /interp_list !list_lookup_fmap.
+          destruct (σ' !! k) as [ t0 | ] eqn:h0 => /=.
+          - destruct (σt !! k) as [ t1 | ] eqn:h1 => /=.
+            + iAssert (interp_type t0 Σt ≡ interp_type t1 Σi)%I as "heq".
+              { by iApply "hinst". }
+              by iRewrite "heq".
+            + apply lookup_ge_None_1 in h1.
+              apply lookup_lt_Some in h0.
+              by lia.
+          - destruct (σt !! k) as [ t1 | ] eqn:h1 => //=.
+            apply lookup_ge_None_1 in h0.
+            apply lookup_lt_Some in h1.
+            by lia.
+        }
+        iRewrite "hctxt".
+        by iSplit; iIntros.
     }
-    iDestruct "hrecv" as (t' def σ' σt' fields ifields) "[%hpure [hsem hl]]".
-    destruct hpure as (hinherits' & hwfσ' & hdef & hσ' & hfields).
+    iDestruct "hrecv" as (t' σ' Σt fields ifields) "[%hpure [#hstatic [#hdyn hl]]]".
+    destruct hpure as (hinherits' & hfields & hdomfields).
     iIntros "#hv hmodels".
     iDestruct "hmodels" as (sh) "[hown [%hdom #h]]".
     iExists sh.
-    iDestruct "hsem" as "[%hdomf #hifields]".
     iDestruct (sem_heap_own_valid_2 with "hown hl") as "#Hv".
-    iSplitL; first by iFrame.
+    iSplitL "hown"; first by iFrame.
     iSplitR.
     { iPureIntro.
       by rewrite hdom dom_insert_lookup_L.
@@ -268,10 +365,10 @@ Section proofs.
     iDestruct "hsh" as "[%ht #hifs]".
     fold_leibniz; subst.
     assert (hfield2 : has_field f rt vis (subst_ty σ' fty) orig) by (by eapply has_field_inherits_using).
-    iSpecialize ("hifields" $! f vis (subst_ty σ' fty) orig hfield2).
-    iAssert (⌜is_Some (iFs !! f)⌝)%I as "%hsome".
+    iSpecialize ("hdyn" $! f vis (subst_ty σ' fty) orig hfield2).
+    iAssert (⌜is_Some (iFs !! f)⌝)%I as "%hiFs".
     { iRewrite -"hifs".
-      by iRewrite "hifields".
+      by iRewrite "hdyn".
     }
     rewrite /heap_models_fields.
     iDestruct "hmodels" as "[%hdomv #hmodfs]".
@@ -287,40 +384,18 @@ Section proofs.
     rewrite lookup_insert.
     iExists v; iSplitR; first done.
     iRewrite -"hifs" in "hf'".
-    iRewrite "hifields" in "hf'".
+    iRewrite "hdyn" in "hf'".
     rewrite !option_equivI later_equivI discrete_fun_equivI.
     iNext.
     iSpecialize ("hf'" $! v).
     iRewrite -"hf'".
-    rewrite subst_ty_subst; last first.
+    rewrite interp_type_subst; last first.
     { apply has_field_bounded in hfield => //.
       destruct hfield as (def' & hdef' & hfty).
-      apply inherits_using_wf in hinherits' => //.
-      destruct hinherits' as (? & ? & ? & hh); inv hh.
-      simplify_eq.
-      by rewrite H4.
+      inv hwf; simplify_eq.
+      by rewrite H2.
     }
-    assert (hsub : Σc ⊢ subst_ty σt fty <: subst_ty (subst_ty σt' <$> σ') fty).
-    { destruct vis.
-      - (* Public field access *)
-        assert (hfwf := hfield).
-        apply has_field_wf in hfwf => //.
-        apply has_field_mono in hfield => //.
-        destruct hfield as (tdef & ? & [_ hcontra]); simplify_eq.
-        apply subtype_lift with (neg_variance <$> generics tdef) => //.
-        + by apply wf_ty_class_inv in hwf.
-        + apply wf_ty_subst_map.
-          * by apply wf_ty_class_inv in hwfσ'.
-          * apply inherits_using_wf in hinherits' => //.
-            destruct hinherits' as (? & ? & ? & hh); by apply wf_ty_class_inv in hh.
-        + by apply neg_subtype_targs.
-      - (* Private field access *)
-        by rewrite hσ'.
-    }
-    iApply subtype_is_inclusion => //.
-    apply has_field_wf in hfield => //.
-    apply wf_ty_subst => //.
-    by apply wf_ty_class_inv in hwf.
+    by iApply "hstatic".
   Qed.
 
   Lemma cmd_adequacy_ Σc lty cmd lty' :
@@ -329,11 +404,11 @@ Section proofs.
     Forall wf_constraint Σc →
     ⌜cmd_has_ty Σc lty cmd lty'⌝ -∗
     ∀ Σi st st' n,
-    ⌜interp_env_as_mixed Σc Σi⌝ →
-    ⌜Σinterp Σc Σi⌝ →
+    ⌜interp_env_as_mixed Σi⌝ →
+    ⌜Σinterp Σi Σc⌝ →
     ⌜cmd_eval st cmd st' n⌝ -∗
-    heap_models st.2 ∗ interp_local_tys Σc Σi lty st.1 -∗ |=▷^n
-        heap_models st'.2 ∗ interp_local_tys Σc Σi lty' st'.1.
+    heap_models st.2 ∗ interp_local_tys Σi lty st.1 -∗ |=▷^n
+        heap_models st'.2 ∗ interp_local_tys Σi lty' st'.1.
   Proof.
     move => wfΔ wflty hΣc .
     iLöb as "IH" forall (Σc lty cmd lty' wflty hΣc).
@@ -387,34 +462,46 @@ Section proofs.
       simpl in *.
       iDestruct "Hle" as "[Hthis Hle]".
       rewrite /this_type /=.
-      iDestruct "Hthis" as (??????) "[%H [#Hifields H◯]]".
-      destruct H as ([= <-] & hinherits & hwfσt & hokσt & htargs & hfields).
-      iAssert (⌜t0 = t1⌝ ∗ heap_models h ∗ ▷ interp_type Σc Σi (subst_ty targs fty) v)%I with "[Hh]" as "[%Ht [Hh Hv]]".
+      rewrite /interp_this_type interp_this_unseal /interp_this_def /=.
+      iDestruct "Hthis" as (??????) "[%H [#hstatic [hdyn H◯]]]".
+      destruct H as ([= <-] & hinherits & hfields & hidom).
+      iAssert (⌜t0 = t1⌝ ∗ heap_models h ∗ ▷ interp_type (subst_ty targs fty) Σi v)%I with "[Hh]" as "[%Ht [Hh Hv]]".
       { iDestruct "Hh" as (sh) "(H● & %hdom & #Hh)".
         iDestruct (sem_heap_own_valid_2 with "H● H◯") as "#HΦ".
         iDestruct ("Hh" with "[//]") as (iFs) "[H H▷]".
         iRewrite "H" in "HΦ".
         rewrite option_equivI prod_equivI /=.
         iDestruct "HΦ" as "[%Ht HΦ]".
-        rewrite -htargs.
         fold_leibniz; subst.
         iSplitR; first done.
         iSplitL. { iExists _. iFrame. by iSplit. }
-        iDestruct "Hifields" as "[%hidom hfields]".
         assert (hfC: has_field name t1 Private (subst_ty σ fty) t) by (destruct wfΔ; by eapply has_field_inherits_using).
-        iSpecialize ("hfields" $! name Private (subst_ty σ fty) t hfC).
+        iSpecialize ("hdyn" $! name Private (subst_ty σ fty) t hfC).
         iDestruct "H▷" as "[%hdf h]".
-        iRewrite -"HΦ" in "hfields".
-        iSpecialize ("h" $! name _ with "[hfields]"); first done.
+        iRewrite -"HΦ" in "hdyn".
+        iSpecialize ("h" $! name _ with "[hdyn]"); first done.
         iDestruct "h" as (w) "[%hw hiw]".
-        rewrite -subst_ty_subst; first by simplify_eq.
-        destruct wfΔ.
-        apply has_field_bounded in hf => //.
-        destruct hf as (? & ? & ?).
-        apply inherits_using_wf in hinherits => //.
-        destruct hinherits as (? & ?& ? & hh).
-        inv hh; simplify_eq.
-        by rewrite H8.
+        iNext; simplify_eq.
+        iSpecialize ("hstatic" $! name Private fty t hf v).
+        assert (bounded (length σ) fty).
+        { destruct wfΔ.
+          apply has_field_bounded in hf => //.
+          destruct hf as (? & ? & ?).
+          apply inherits_using_wf in hinherits => //.
+          destruct hinherits as (? & ?& ? & hh).
+          inv hh; simplify_eq.
+          by rewrite H8.
+        }
+        assert (bounded (length targs) fty).
+        { destruct wfΔ.
+          apply has_field_bounded in hf => //.
+          destruct hf as (? & ? & ?).
+          inv wfthis; simplify_eq.
+          by rewrite H5.
+        }
+        rewrite !interp_type_subst //.
+        iRewrite "hstatic".
+        iApply interp_type_subst => //.
       }
       subst.
       iNext.
@@ -422,19 +509,20 @@ Section proofs.
       iApply interp_local_tys_update => //.
       iSplit; last done.
       rewrite /type_of_this /=.
-      iExists l, t1, σ, σt, fields, ifields.
-      iSplit.
-      + iPureIntro; by (repeat split => //).
-      + by iSplit.
+      rewrite /interp_this_type interp_this_unseal /interp_this_def /=.
+      iExists l, t1, σ, Σt, fields, ifields.
+      iSplit; first done.
+      iSplitR; first done.
+      by iSplit.
     - (* GetC *) inv hc.
       iClear "IH".
       iIntros "[Hh #Hle]".
       iModIntro. (* keep the later *)
       iDestruct (expr_adequacy with "Hle") as "#He" => //; try (by apply wfΔ).
-      rewrite interp_class_unfold /=.
-      iDestruct "He" as (???????) "[%H [#Hifields H◯]]".
-      destruct H as ([= <-] & hinherits & hwfσt & hokσt & hdef & htargs & hfields).
-      iAssert (⌜t0 = t1⌝ ∗ heap_models h ∗ ▷ interp_type Σc Σi (subst_ty (subst_ty σt <$> σ)  fty) v)%I with "[Hh]" as "[%Ht [Hh Hv]]".
+      rewrite !interp_class_unfold !interp_tag_unseal /interp_tag_def /interp_fun !interp_car_simpl /=.
+      iDestruct "He" as (??? Σt ??) "[%H [#hstatic [#hdyn H◯]]]".
+      destruct H as ([= <-] & hinherits & hfields & hidom).
+      iAssert (⌜t0 = t1⌝ ∗ heap_models h ∗ ▷ interp_type (subst_ty σ  fty) Σt v)%I with "[Hh]" as "[%Ht [Hh Hv]]".
       { iDestruct "Hh" as (sh) "(H● & %hdom & #Hh)".
         iDestruct (sem_heap_own_valid_2 with "H● H◯") as "#HΦ".
         iDestruct ("Hh" with "[//]") as (iFs) "[H H▷]".
@@ -444,44 +532,29 @@ Section proofs.
         fold_leibniz; subst.
         iSplitR; first done.
         iSplitL. { iExists _. iFrame. by iSplit. }
-        iAssert (interp_fields t (subst_ty σt <$> σ) (dom fields) ifields (interp_type Σc Σi)) with "[Hifields]" as "Hifields_t".
-        { destruct wfΔ.
-          by iApply interp_fields_inclusion.
-        }
-        rewrite /interp_fields.
-        iDestruct "Hifields_t" as "[%hdiom Hifields_t]".
-        iSpecialize ("Hifields_t" $! name Public fty orig hf).
+        assert (hf2 := hf).
+        apply has_field_inherits_using with (A := t1) ( σB := σ) in hf2 => //; (try by apply wfΔ).
+        iSpecialize ("hdyn" $! name Public (subst_ty σ fty) orig hf2).
         iDestruct "H▷" as "[%hdf h]".
-        iRewrite -"HΦ" in "Hifields_t".
-        iSpecialize ("h" $! name _ with "[Hifields_t]"); first done.
-        iDestruct "h" as (w) "[%hw hiw]".
+        iRewrite -"HΦ" in "hdyn".
+        iDestruct ("h" with "hdyn") as (w) "[%hw hiw]".
         by simplify_eq.
       }
       subst.
       iNext.
+      rewrite -/interp_local_tys.
       iFrame.
-      destruct wfΔ.
-      assert (hsub: Σc ⊢ subst_ty (subst_ty σt <$> σ) fty <: subst_ty targs fty).
-      { assert (hfwf := hf).
-        apply has_field_wf in hfwf => //.
-        apply has_field_mono in hf => //.
-        destruct hf as (tdef & ? & [hcov _]); simplify_eq.
-        apply subtype_lift with (generics tdef) => //.
-        - apply wf_ty_subst_map; first by apply wf_ty_class_inv in hwfσt.
-          apply inherits_using_wf in hinherits => //.
-          destruct hinherits as (? & ? & ? & hh).
-          by apply wf_ty_class_inv in hh.
-        - apply expr_has_ty_wf in hrecv => //.
-          by apply wf_ty_class_inv in hrecv.
-      }
+      iSpecialize ("hstatic" $! name fty orig hf v).
       iApply interp_local_tys_update => //.
-      iApply subtype_is_inclusion => //.
-      apply wf_ty_subst.
-      * apply wf_ty_subst_map; first by apply wf_ty_class_inv in hwfσt.
-        apply inherits_using_wf in hinherits => //.
-        destruct hinherits as (? & ? & ? & hh).
-        by apply wf_ty_class_inv in hh.
-      * by apply has_field_wf in hf.
+      rewrite (interp_type_subst Σi fty targs); last first.
+      { apply has_field_bounded in hf; try (by apply wfΔ).
+        destruct hf as (hdef & htdef & hb).
+        apply expr_has_ty_wf in hrecv => //.
+        inv hrecv; simplify_eq.
+        by rewrite H2.
+      }
+      by iApply "hstatic".
+    - admit (*
     - (* SetPriv *) inv hc.
       assert (wfΔ' := wfΔ).
       destruct wfΔ'.
@@ -501,6 +574,8 @@ Section proofs.
         repeat iSplit => //.
         by inv H2.
       + iApply expr_adequacy => //; by apply wfΔ.
+             *).
+    - admit (*
     - (* SetPub *) inv hc.
       assert (wfΔ' := wfΔ).
       destruct wfΔ'.
@@ -511,7 +586,9 @@ Section proofs.
       iApply heap_models_update => //.
       + iApply expr_adequacy => //; by apply wfΔ.
       + iApply expr_adequacy => //; by apply wfΔ.
+             *).
     - (* NewC *) inv hc.
+      iClear "IH".
       iIntros "[Hh #Hle]"; simpl.
       (* we need one modality to semantic heap *)
       iDestruct "Hh" as (sh) "(H● & %Hdom & #Hh)".
@@ -519,31 +596,61 @@ Section proofs.
       { apply (not_elem_of_dom (D:=gset loc)).
         by rewrite Hdom not_elem_of_dom.
       }
+      (* Let's interpret the types of all fields/arguments *)
       set (iFs :=
-         (λ(ty: lang_ty), Next (interp_car (interp_type Σc Σi ty))) <$> ((λ x, subst_ty targs x.1.2) <$> fields)
+         (λ(ty: lang_ty), Next (interp_car (interp_type ty Σi))) <$> ((λ x, subst_ty targs x.1.2) <$> fields)
       ).
       iMod ((sem_heap_own_update new) with "H●") as "[H● #H◯]" => //;
         first by apply (sem_heap_view_alloc _ new t iFs).
       iIntros "!> !>". (* kill the modalities *)
-      iAssert (interp_type Σc Σi (ClassT t targs) (LocV new)) with "[]" as "#Hl".
+      iAssert (interp_type (ClassT t targs) Σi (LocV new)) with "[]" as "#Hl".
       {
-        iAssert (interp_fields t targs (dom fields) iFs (interp_type Σc Σi)) as "HiFs".
-        { rewrite /interp_fields; iSplit; first by rewrite /iFs !dom_fmap_L.
-          iIntros (f vis fty orig) "%hfty".
-          apply hf in hfty.
-          rewrite /iFs !lookup_fmap.
-          by rewrite hfty /=.
-        }
-        rewrite interp_type_unfold /=.
+        rewrite !interp_class_unfold !interp_tag_unseal /interp_tag_def /interp_fun !interp_car_simpl /=.
         assert (hwf' := hwf).
         inv hwf'.
-        iExists new, t, def, (gen_targs (length def.(generics))), targs, fields, iFs.
-        iSplit; last by (repeat iSplit => //).
-        iPureIntro.
-        repeat split => //.
-        + by econstructor.
-        + rewrite subst_ty_gen_targs => //.
-          by apply subtype_targs_refl.
+        iExists new, t, (gen_targs (length def.(generics))), (interp_list Σi targs), fields, iFs.
+        iSplit.
+        { iPureIntro; repeat split => //.
+          + by econstructor.
+          + by rewrite !dom_fmap_L.
+        }
+        iSplit.
+        { iModIntro; iNext.
+          iIntros (f ty orig hhf v).
+          (* TODO CLEAN UP *)
+          iAssert (interp_type ty ((λ ty0 : lang_ty, interp_type ty0 Σi) <$> targs) v ∗-∗
+                   interp_type (subst_ty (gen_targs (length (generics def))) ty) (interp_list Σi targs) v)%I as "HH".
+          { rewrite interp_type_subst; last first.
+            { apply has_field_bounded in hhf; try (by apply wfΔ).
+              destruct hhf as (? & ? & hb).
+              rewrite length_gen_targs.
+              by simplify_eq.
+            }
+            rewrite interp_list_gen_targs; last first.
+            { by rewrite /interp_list fmap_length. }
+            pose (hh := interp_list_fold Σi targs).
+            apply interp_type_equivI with (ty := ty) (v := v) in hh.
+            rewrite -hh.
+            by iSplit; iIntros.
+          }
+          done.
+        }
+        iSplit; last done.
+        iIntros (f vis ty orig hfty).
+        apply hf in hfty.
+        rewrite /iFs !lookup_fmap hfty /=.
+        rewrite option_equivI later_equivI.
+        iNext.
+        rewrite discrete_fun_equivI.
+        iIntros (w).
+        iAssert (interp_type (subst_ty targs ty) Σi w ≡ interp_type ty (interp_list Σi targs) w)%I as "H".
+        { rewrite interp_type_subst //.
+          apply hf in hfty.
+          apply has_field_bounded in hfty; try (by apply wfΔ).
+          destruct hfty as (? & ? & hb); simplify_eq.
+          by rewrite H2.
+        }
+        done.
       }
       iSplitL; last by iApply interp_local_tys_update.
       iExists _. iFrame. iSplit; first by rewrite !dom_insert_L Hdom.
@@ -585,13 +692,13 @@ Section proofs.
       assert (h2: is_Some (fields !! f)) by (by apply elem_of_dom).
       destruct h2 as [fty hty].
       iExists v0; iSplitR; first done.
-      rewrite /interp_fields lookup_fmap.
+      rewrite !lookup_fmap.
       assert (heval0: expr_eval le a0 = Some v0).
       { rewrite (map_args_lookup _ _ _ args vargs H6 f) in hv0.
         by rewrite ha0 in hv0.
       }
       assert (hty0: expr_has_ty Σc lty a0 (subst_ty targs fty.1.2)) by (by apply harg with f).
-      rewrite !lookup_fmap hty /=  option_equivI later_equivI.
+      rewrite hty /=  option_equivI later_equivI.
       iNext.
       rewrite discrete_fun_equivI.
       iSpecialize ("hiF" $! v0).
@@ -612,9 +719,9 @@ Section proofs.
       rename H12 into heval_ret.
       (* Get inherits relation between dynamic tag and static tag *)
       iDestruct (expr_adequacy Σc Σi recv with "Hle") as "#Hrecv" => //.
-      rewrite interp_class_unfold /=.
-      iDestruct "Hrecv" as (? t1 def σin σt fields ifields) "[%Hpure [hifields Hl]]".
-      destruct Hpure as ([= <-] & hin_t1_t & hwf_t1_σt & hok_t1_σt & hdef & htargs & hfields).
+      rewrite interp_class_unfold interp_tag_unseal /interp_tag_def /=.
+      iDestruct "Hrecv" as (? t1 σin Σt fields ifields) "[%Hpure [#hstatic [#hdyn Hl]]]".
+      destruct Hpure as ([= <-] & hin_t1_t & hfields & hidom).
       iDestruct "Hh" as (sh) "(H● & %Hdom & #Hh)".
       iDestruct (sem_heap_own_valid_2 with "H● Hl") as "#HΦ".
       iDestruct ("Hh" with "[//]") as (?) "[H H▷]".
@@ -622,22 +729,328 @@ Section proofs.
       rewrite option_equivI prod_equivI /=.
       iDestruct "HΦ" as "[%Ht HΦ]".
       fold_leibniz; subst.
-      (* both static and dynamic classes actually exists in Δ *)
-      assert (ht1: is_Some (Δ !! t1)).
-      { apply has_method_from_def in hhasm0 as (? & ? & ? & ? & _ & [? [hin ?]]) => //.
-        by apply inherits_using_wf in hin as (? & ? & ht1 & _).
-      }
-      destruct ht1 as [ def1 hdef1 ].
+      (***********************)
       (* Get method inclusion information between mdef0 and mdef *)
       destruct (has_method_ordered _ _ _ _ _ _ _ _
-        wf_extends_wf wf_override wf_parent wf_methods_bounded
-        hin_t1_t hhasm0 hhasm)
-      as (σoin & σot1 & σot & odef0 & odef & omdef0 & omdef &
-         hσeq & hodef0 & hodef & homdef0 & homdef & hin_o0_o & hin_t1_o0 & hin_t_o &
-         -> & -> & hincl0 & hincl1).
-      (* Get location of the definition of the dynamic method mdef0 *)
-      destruct (has_method_from_def _ _ _ _  wf_parent wf_methods_bounded hhasm0) as
-        (odef0' & mdef0_orig & hodef0' & hmdef0_orig & hhasm_morig0 & [σ0 [hin_t1_o0' heqmdef]]).
+        wf_extends_wf wf_override wf_parent wf_methods_bounded hin_t1_t hhasm0 hhasm)
+      as (odef0 & odef & σt1_o0 & σt_o & omdef0 & omdef & hodef0 & hodef &
+        homdef0 & homdef & hin_t1_o0 & hin_t_o & -> & -> & hincl0 & hmeth).
+      (* omdef0 is well typed *)
+      assert (hwfo0: wf_ty (ClassT orig0 σt1_o0)) by admit.
+      assert (hoko0: ok_ty odef0.(constraints) (ClassT orig0 σt1_o0)) by admit.
+      destruct (wf_mdef_ty_gen _ _ _ _ _ _ wfΔ hodef0 homdef0 hwfo0 hoko0)
+        as (rty & hwfrty & hbody & hret).
+      iModIntro; iNext.
+      assert (hwflty: wf_lty {| type_of_this := (orig0, σt1_o0);
+                               ctxt := subst_ty σt1_o0 <$> methodargs omdef0 |}).
+      admit.
+      assert (hΣ0 : Forall wf_constraint odef0.(constraints)) by admit.
+      assert (hΣt : interp_env_as_mixed Σt) by admit (* TODO: add that to interp *).
+      assert (hΣ0Σt : Σinterp Σt odef0.(constraints)) by admit (* TODO: add that to interp *).
+      iSpecialize ("IH" $! _ _ _ _ hwflty hΣ0 hbody Σt _ _ _ hΣt hΣ0Σt heval_body); simpl.
+      iDestruct ("IH" with "[Hh Hle H●]") as "Hstep".
+      { iSplit.
+        { iExists _; iFrame.
+          iSplit; last done.
+          by rewrite Hdom.
+        }
+        iSplit => /=.
+        - rewrite /interp_this_type interp_this_unseal /interp_this_def /=.
+          iExists l, t1, σt1_o0, Σt, fields, ifields.
+          iSplit; first by iPureIntro.
+          iSplit; last by iSplit.
+          iModIntro; iNext.
+          iIntros (f vis ty o hf v).
+          rewrite interp_type_subst //.
+          admit.
+        - iIntros (v ty hin).
+          rewrite lookup_fmap_Some in hin.
+          destruct hin as [ty' [<- hx]].
+          assert (ha: ∃ arg, args !! v = Some arg).
+          { apply elem_of_dom.
+            destruct hincl0 as [hh _].
+            rewrite /subst_mdef /= !dom_fmap_L in hh.
+            rewrite -hdom /subst_mdef /= dom_fmap -hh.
+            apply elem_of_dom.
+            now rewrite hx.
+          }
+          destruct ha as [arg harg].
+          assert (hv: ∃ varg, vargs !! v = Some varg).
+          { apply elem_of_dom.
+            apply dom_map_args in hmap.
+            rewrite hmap.
+            apply elem_of_dom.
+            now rewrite harg.
+          }
+          destruct hv as [varg hvarg].
+          iExists varg; iSplit; first done.
+          apply helt with v ty arg in hin; last done.
+
+
+
+
+
+
+
+    move => ?????????? hdom hargs helt.
+    iIntros "#Hl #[Hthis Hle]".
+    iSplit; first done.
+    iIntros (v ty) "%hin".
+    assert (ha: ∃ arg, args !! v = Some arg).
+    { apply elem_of_dom.
+      rewrite -hdom.
+      apply elem_of_dom.
+      now rewrite hin.
+    }
+    destruct ha as [arg harg].
+    apply helt with v ty arg in hin; last done.
+    assert (hv: ∃ varg, vargs !! v = Some varg).
+    { apply elem_of_dom.
+      apply dom_map_args in hargs.
+      rewrite hargs.
+      apply elem_of_dom.
+      now rewrite harg.
+    }
+    destruct hv as [varg hvarg].
+    iExists varg; rewrite hvarg; iSplitR; first done.
+    rewrite (map_args_lookup _ _ _ args vargs hargs v) harg /= in hvarg.
+    iApply expr_adequacy => //.
+    by iSplit.
+  Qed.
+
+      }
+      iRevert "Hstep".
+      iApply updN_mono_I.
+      iIntros "[Hmodels Hle2]"; iFrame.
+      iApply interp_local_tys_update; first by done.
+      destruct hincl1 as [? [? hret1]].
+      assert (hsub: Σc ⊢ subst_ty (subst_ty σt <$> σ0) (methodrettype omdef0) <:
+                         subst_ty targs (subst_ty σot (methodrettype omdef))).
+      { eapply SubTrans; last first.
+        - apply subtype_lift with (σ0 := subst_ty σt <$> σin) (vs := generics def) => //.
+          + assert (hmono := hodef).
+            apply wf_methods_mono in hmono.
+            assert (hm := homdef).
+            apply hmono in hm as [_ hmonoret].
+            apply mono_subst with (generics odef) => //.
+            * apply wf_methods_bounded in hodef.
+              apply hodef in homdef.
+              by apply homdef.
+            * apply inherits_using_wf in hin_t_o => //.
+              repeat destruct hin_t_o as [? hin_t_o]; inv hin_t_o; by simplify_eq.
+            * move => i vi ti hvi hti hc.
+              apply inherits_using_mono with (def := def) in hin_t_o => //.
+              inv hin_t_o; simplify_eq.
+              by eauto.
+            * move => i vi ti hvi hti hc.
+              apply inherits_using_mono with (def := def) in hin_t_o => //.
+              inv hin_t_o; simplify_eq.
+              by eauto.
+          + apply wf_ty_subst => //.
+            * apply inherits_using_wf in hin_t_o => //.
+              repeat destruct hin_t_o as [? hin_t_o]; by apply wf_ty_class_inv in hin_t_o.
+            * apply wf_methods_wf in hodef.
+              apply hodef in homdef.
+              by apply homdef.
+        - rewrite -!subst_ty_subst //.
+          + apply wf_methods_ok in hodef0.
+            apply hodef0 in homdef0 as [_ hret_ok].
+            apply subtype_subst with (σ := σt) in hret1 => //.
+            apply subtype_weaken
+              with (Γ' := Σc ++ subst_constraints σt (def1.(constraints) ++ subst_constraints σ0 odef0.(constraints)))
+              in hret1 => //;
+              last by set_solver.
+            by apply subtype_constraint_elim in hret1.
+          + apply bounded_subst with (length σot) => //.
+            apply inherits_using_wf in hin_t_o => //.
+            destruct hin_t_o as (? & ? & ? & hh); inv hh.
+            simplify_eq.
+            assert (ho := hodef).
+            apply wf_methods_bounded in ho.
+            apply ho in homdef.
+            rewrite H6.
+            by apply homdef.
+      }
+      iDestruct (expr_adequacy Σc Σi (methodret omdef0) with "Hle2") as "#Hret" => //.
+      iApply subtype_is_inclusion => //.
+      + apply wf_ty_subst.
+       * by apply wf_ty_subst_map.
+       * apply wf_methods_wf in hodef0.
+         apply hodef0 in homdef0.
+         by apply homdef0.
+      + by rewrite -subst_ty_subst.
+    
+
+
+
+      { iClear "IH".
+        iSplit.
+        - iExists _; iFrame.
+          iSplit; last done.
+          by rewrite Hdom.
+        - iApply (interp_local_tys_list _ _ lty le) => //.
+          + destruct hincl0 as [hdomincl _].
+            rewrite !dom_fmap_L in hdomincl.
+            rewrite !dom_fmap_L in hdom.
+            by rewrite !dom_fmap_L hdom.
+          + move => x ty arg.
+            rewrite lookup_fmap_Some /=.
+            case => [tx [<- ]] hx harg.
+            assert (hhx: methodargs (subst_mdef σt_o omdef) !! x = Some (subst_ty σt_o tx)).
+            { by rewrite /subst_mdef /= lookup_fmap hx. }
+            move : (hi x (subst_ty σt_o tx) arg hhx harg) => hargty.
+            rewrite -subst_ty_subst //.
+            assert (h0 := hodef).
+            apply wf_methods_bounded in hodef.
+            apply hodef in homdef.
+            apply homdef in hx.
+            apply inherits_using_wf in hin_t_o => //.
+            destruct hin_t_o as (? & ? & ? & hh).
+            inv hh; simplify_eq.
+            by rewrite H4.
+          + rewrite /interp_this_type interp_this_unseal /interp_this_def /=.
+            iExists l, t1, σt1_o0, Σi, fields, ifields.
+            iSplit; first by iPureIntro.
+            iSplit.
+            * iModIntro; iNext.
+              iIntros (f vis ty o hf v).
+              rewrite interp_type_subst //.
+              apply has_field_bounded in hf => //.
+              destruct hf as (? & ? & hf); simplify_eq.
+              apply inherits_using_wf in hin_t1_o0 => //.
+              destruct hin_t1_o0 as (? & ? &? & hwf).
+              inv hwf; simplify_eq.
+              by rewrite H4.
+            * iSplit; last done.
+              assert (h0 := hodef0).
+              apply wf_methods_bounded in hodef.
+            apply hodef in homdef.
+            apply homdef in hx.
+            apply inherits_using_wf in hin_t_o => //.
+            destruct hin_t_o as (? & ? & ? & hh).
+            inv hh; simplify_eq.
+            by rewrite H4.
+
+              * apply hi with x => //.
+              rewrite /subst_mdef /= lookup_fmap hx'.
+            
+bounded (length σt_o) tx
+            { by rewrite /subst_mdef /= lookup_fmap hx'. }
+            eapply ESubTy; first by apply hargty.
+            admit.
+            admit.
+            destruct hmeth as [hmeth | hmeth].
+            * destruct hmeth as ( ? & -> & -> & <-).
+              rewrite hx in hx'; simplify_eq.
+              apply SubRefl.
+                by rewrite hx in hx'.
+              * destruct hmeth as (σ & ? & <- & hincl1).
+            by elim hx.
+            destruct (methodargs omdef !! x) as [ty' | ] eqn:hty'.
+            { assert (bounded (length σot) ty').
+              { assert (ho := hodef).
+                apply wf_methods_bounded in ho.
+                apply ho in homdef.
+                apply homdef in hty'.
+                apply inherits_using_wf in hin_t_o => //.
+                destruct hin_t_o as ( ? & ? & ? & hh); inv hh; simplify_eq.
+                by rewrite H4.
+              }
+            { Search lookup 
+
+            assert (methodargs (subst_mdef σt_o omdef) !! x = Some (subst_ty σt_o ty)).
+            { rewrite /subst_mdef /= lookup_fmap .
+
+hi : ∀ (x : string) (ty : lang_ty) (arg : expr),
+       methodargs (subst_mdef σt_o omdef) !! x = Some ty
+       → args !! x = Some arg → expr_has_ty Σc lty arg (subst_ty targs ty)
+  Lemma interp_local_tys_list Σc Σi lty le targs args vargs l t σ:
+    map_Forall (λ _cname, wf_cdef_fields) Δ →
+    map_Forall (λ _ : string, wf_cdef_fields_wf) Δ →
+    map_Forall (λ _cname, wf_cdef_fields_bounded) Δ →
+    map_Forall (λ _cname, wf_cdef_parent Δ) Δ →
+    map_Forall (λ _ : string, wf_cdef_mono) Δ →
+    map_Forall (λ _ : string, wf_field_mono) Δ → 
+    Σinterp Σi Σc →
+    interp_env_as_mixed Σi →
+    Forall wf_constraint Σc →
+    wf_lty lty →
+    dom targs = dom args →
+    map_args (expr_eval le) args = Some vargs →
+    (∀ (x : string) (ty : lang_ty) (arg : expr),
+    targs !! x = Some ty →
+    args !! x = Some arg →
+    expr_has_ty Σc lty arg ty) →
+    interp_this_type t σ Σi (LocV l) -∗
+    interp_local_tys Σi lty le -∗
+    interp_local_tys Σi {| type_of_this := (t, σ); ctxt := targs |}
+                        {| vthis := l; lenv := vargs |}.
+
+
+
+
+      assert (ho0 := hodef0).
+      assert (hm0 := homdef0).
+      apply wf_mdefs in ho0.
+      apply ho0 in hm0.
+      destruct hm0 as (rty0 & hwf_rty0 & hbody0 & hret0).
+      assert (hwflty0: wf_lty
+           {|
+             type_of_this := (orig0, σt1_o0);
+             ctxt :=
+               subst_ty σt1_o0 <$> methodargs omdef0
+           |}
+           ) by admit.
+      iModIntro; iNext.
+      iSpecialize ("IH" $! _ _ _ _ hwflty0 hΣc hbody0 Σi _ _ _ hΣi hΣcΣi heval_body); simpl.
+      iDestruct ("IH" with "[Hh Hle H●]") as "Hstep".
+      { iSplit.
+        - iExists _; iFrame.
+          iSplit; last done.
+          by rewrite Hdom.
+        - iApply (interp_local_tys_list _ _ lty le) => //.
+          + destruct hincl0 as [hdomincl _].
+            rewrite !dom_fmap_L in hdomincl.
+            rewrite !dom_fmap_L in hdom.
+            by rewrite !dom_fmap_L hdomincl hdom.
+          + move => x ty arg.
+            rewrite lookup_fmap_Some /=.
+            case => [tx [<- ]] hx harg.
+            destruct hmeth as [hmeth | hmeth].
+            * destruct hmeth as (hin_t_o0 & -> & -> & <-).
+                by rewrite hx.
+              - destruct hmeth as (σ & hσ & <- & hincl2).
+                destruct hincl2 as [? hincl2].
+
+
+
+
+
+            pose (hty := hi x ty arg _ harg
+
+hi : ∀ (x : string) (ty : lang_ty) (arg : expr),
+       methodargs (subst_mdef σt_o omdef) !! x = Some ty
+       → args !! x = Some arg → expr_has_ty Σc lty arg (subst_ty targs ty)
+expr_has_ty Σc lty arg (subst_ty σt1_o0 tx)
+
+            (* 
+
+hi : ∀ (x : string) (ty : lang_ty) (arg : expr),
+       methodargs (subst_mdef σt_o omdef) !! x = Some ty
+       → args !! x = Some arg → expr_has_ty Σc lty arg (subst_ty targs ty)
+             *)
+
+
+            rewrite lookup_fmap_Some.
+            case => [tx' [<- hx]] harg.
+            destruct hincl1 as [hdom1 [hincl1 _]].
+            destruct (methodargs omdef !! x) as [ty' | ] eqn:hty'.
+
+
+
+
+
+
       assert (hokσ0: Forall (ok_ty def1.(constraints)) σ0).
       { apply inherits_using_ok in hin_t1_o0' => //.
         destruct hin_t1_o0' as (? & ? & hok); simplify_eq.
@@ -662,8 +1075,6 @@ Section proofs.
         destruct hin_t1_t as (? & ? & ? &hh).
         by apply wf_ty_class_inv in hh.
       }
-      assert (hwf_σt: Forall wf_ty σt) by (by apply wf_ty_class_inv in hwf_t1_σt).
-      assert (hwf_σt_σin: Forall wf_ty (subst_ty σt <$> σin)) by (by apply wf_ty_subst_map).
       assert (hb_σin_σot : Forall (bounded (length σin)) σot).
       { apply inherits_using_wf in hin_t1_t => //.
         destruct hin_t1_t as (? & ? & ? &hh).
